Array.v
@@ -1,0 +1,213 @@
+From Coq Require Import Arith NArith Lia.
+
+From Vyper Require Import List2.
+
+Local Open Scope list_scope.
+
+(** An typical array container. Coq's standard [Vector] is very similar to this. *)
+Class class {Value: Type} (Zero: Value) (length: N) (A: Type) := {
+  get: A -> forall i: N, (i < length)%N -> Value;
+  zeros: A;
+
+  zeros_ok: forall (i: N) (Ok: (i < length)%N),
+              get zeros i Ok = Zero;
+
+  put: A -> forall (i: N) (Ok: (i < length)%N), Value -> A;
+
+  put_ok: forall (a: A) (n: N) (OkN: (n < length)%N) (k: N) (OkK: (k < length)%N) (v: Value),
+            get (put a n OkN v) k OkK
+             =
+            if (n =? k)%N
+              then v
+              else get a k OkK;
+
+  to_list: A -> list Value;
+
+  to_list_ok: forall (a: A) (n: N) (OkN: (n < length)%N),
+                get a n OkN = List.nth (N.to_nat n) (to_list a) Zero;
+
+  to_list_len: forall (a: A),
+                 List.length (to_list a) = N.to_nat length;
+
+  from_list: forall (l: list Value) (Ok: List.length l = N.to_nat length), A;
+  from_list_ok: forall (l: list Value) (OkL: List.length l = N.to_nat length)
+                       (n: N) (OkN: (n < length)%N),
+                  get (from_list l OkL) n OkN = List.nth (N.to_nat n) l Zero;
+
+  (** Given an offset and a count, convert the corresponding subarray to a list. *)
+  view: A -> forall (offset count: N) (Ok: (offset + count <= length)%N), list Value;
+  view_len: forall (a: A) (offset count: N) (Ok: (offset + count <= length)%N),
+              List.length (view a offset count Ok) = N.to_nat count;
+  view_ok: forall (a: A) (offset count: N) (Ok: (offset + count <= length)%N)
+                  (n: N) (OkN: (n < count)%N) (Ok': (offset + n < length)%N),
+             List.nth_error (view a offset count Ok) (N.to_nat n) = Some (get a (offset + n)%N Ok');
+}.
+
+Lemma put_same {Value: Type} {Zero: Value} {A: Type} (len: N) (C: class Zero len A)
+               (a: A) (n: N) (OkN: (n < len)%N) (v: Value):
+  get (put a n OkN v) n OkN = v.
+Proof.
+rewrite put_ok.
+enough (H: (n =? n)%N = true) by now rewrite H.
+now apply N.eqb_eq.
+Qed.
+
+
+Section ListInst.
+  Context {Value: Type} (Zero: Value) (len: N).
+
+  Definition t := { l : list Value | List.length l = N.to_nat len }.
+
+  Definition list_get (a: t) (n: N) (Ok: (n < len)%N)
+  : Value
+  := List.nth (N.to_nat n) (proj1_sig a) Zero.
+
+  Definition list_zeros
+  : t
+  := exist _ (List.repeat Zero (N.to_nat len)) (List.repeat_length _ _).
+
+  Lemma list_zeros_ok (i: N) (Ok: (i < len)%N):
+     list_get list_zeros i Ok = Zero.
+  Proof.
+  cbn. clear Ok.
+  remember (N.to_nat i) as k. clear Heqk i.
+  remember (N.to_nat len) as n. clear Heqn len.
+  revert k.
+  induction n as [|n]; intro k; destruct k as [|k]; try easy.
+  cbn.
+  apply IHn.
+  Qed.
+
+  Local Lemma list_put_helper (a: t) (n: N) (Ok: (n < len)%N) (v: Value):
+    let i := N.to_nat n in
+    let l := proj1_sig a in
+    List.length (List.firstn i l ++ v :: List.skipn (S i) l) = N.to_nat len.
+  Proof.
+  cbn.
+  assert (OkA := proj2_sig a). cbn in OkA.
+  rewrite List.app_length.
+  rewrite List.firstn_length_le by lia.
+  cbn.
+  destruct (proj1_sig a). { cbn in *. lia. }
+  cbn in OkA.
+  rewrite List.skipn_length. lia.
+  Qed.
+
+  Definition list_put (a: t) (n: N) (Ok: (n < len)%N) (v: Value)
+  : t
+  := let i := N.to_nat n in
+     let l := proj1_sig a in
+     exist _ (List.firstn i l ++ v :: List.skipn (S i) l) (list_put_helper a n Ok v).
+
+  Lemma list_put_ok (a: t) (n: N) (OkN: (n < len)%N) (k: N) (OkK: (k < len)%N) (v: Value):
+    list_get (list_put a n OkN v) k OkK = (if (n =? k)%N then v else list_get a k OkK).
+  Proof.
+  cbn.
+  remember (n =? k)%N as e.
+  apply N.compare_lt_iff in OkN.
+  (* apply N.compare_lt_iff in OkK. <- interesting example of deptypes making a weird error *)
+  rewrite N2Nat.inj_compare in OkN.
+  rewrite N.eqb_compare in Heqe.
+  rewrite N2Nat.inj_compare in Heqe.
+  rewrite<- Nat.eqb_compare in Heqe.
+  apply nat_compare_lt in OkN.
+  unfold list_get.
+  apply N.compare_lt_iff in OkK.
+  rewrite N2Nat.inj_compare in OkK.
+  apply nat_compare_lt in OkK.
+  remember (N.to_nat k) as k'. clear k Heqk'. rename k' into k.
+  remember (N.to_nat n) as n'. clear n Heqn'. rename n' into n.
+  assert (OkA := proj2_sig a). cbn in OkA.
+  destruct (proj1_sig a) as [|head]. { cbn in *. lia. } clear a.
+  remember (N.to_nat len) as len'. clear len Heqlen'. rename len' into len.
+  revert head len OkA n OkN k OkK e Heqe. induction l; intros; cbn.
+  {
+    rewrite List.skipn_nil. cbn in OkA. subst len.
+    assert (n = 0) by lia; subst.
+    assert (k = 0) by lia; subst.
+    easy.
+  }
+  cbn in OkA.
+  destruct n as [|n'], k as [|k']; cbn in *; subst; try easy.
+  apply lt_S_n in OkN. apply lt_S_n in OkK.
+  apply (IHl a (S (length l)) eq_refl n' OkN k' OkK (n' =? k') eq_refl).
+  Qed.
+
+  Definition list_view (a: t) (offset count: N)
+  : list Value
+  := List.firstn (N.to_nat count) (List.skipn (N.to_nat offset) (proj1_sig a)).
+
+  Lemma list_view_len (a: t) (offset count: N) (Ok: (offset + count <= len)%N):
+    List.length (list_view a offset count) = N.to_nat count.
+  Proof.
+  unfold list_view.
+  apply List.firstn_length_le.
+  rewrite List.skipn_length.
+  assert (OkA := proj2_sig a). cbn in OkA.
+  rewrite OkA.
+  lia.
+  Qed.
+
+  Lemma list_view_ok (a: t) (offset count: N) (Ok: (offset + count <= len)%N)
+                     (n: N) (OkN: (n < count)%N) (OkSum : (offset + n < len)%N):
+    List.nth_error (list_view a offset count) (N.to_nat n) = Some (list_get a (offset + n) OkSum).
+  Proof.
+  unfold list_view. unfold list_get.
+  assert (OkL := proj2_sig a). cbn in OkL.
+  remember (proj1_sig a) as l. clear Heql a.
+
+  apply N.compare_lt_iff in OkN.
+  apply N.compare_lt_iff in OkSum.
+  apply N.compare_le_iff in Ok.
+
+  rewrite N2Nat.inj_compare in *.
+  rewrite N2Nat.inj_add in *.
+  remember (N.to_nat n) as n'. clear n Heqn'. rename n' into n.
+  remember (N.to_nat count) as count'. clear count Heqcount'. rename count' into count.
+  remember (N.to_nat offset) as offset'. clear offset Heqoffset'. rename offset' into offset.
+  remember (N.to_nat len) as len'. clear len Heqlen'. rename len' into len.
+
+  apply nat_compare_lt in OkSum.
+  apply nat_compare_lt in OkN.
+  apply nat_compare_le in Ok.
+
+  revert len OkL offset count n Ok OkSum OkN. induction l as [|head]; intros.
+  { cbn in OkL. subst. lia. }
+  cbn.
+  destruct count. { lia. }
+  cbn.
+  destruct offset; cbn.
+  {
+    destruct n. { easy. }
+    cbn. cbn in OkL.
+    rewrite List.nth_error_nth' with (d := Zero). 2:{ rewrite List.firstn_length_le; lia. }
+    f_equal.
+    apply nth_firstn.
+    lia.
+  }
+  cbn in OkL.
+  assert (SL := List.skipn_length offset l).
+  remember (List.skipn offset l) as s.
+  destruct s. { cbn in SL. lia. }
+  rewrite<- (IHl (length l) eq_refl offset (S count)); try lia.
+  now rewrite<- Heqs.
+  Qed.
+
+  Definition list_inst
+  : class Zero len t
+  := {| get := list_get
+      ; zeros := list_zeros
+      ; zeros_ok := list_zeros_ok
+      ; put := list_put
+      ; put_ok := list_put_ok
+      ; to_list a := proj1_sig a
+      ; to_list_ok a n OkN := eq_refl
+      ; to_list_len a := proj2_sig a
+      ; from_list := exist _
+      ; from_list_ok a n k OkK := eq_refl
+      ; view a offset count _ := list_view a offset count
+      ; view_len := list_view_len
+      ; view_ok := list_view_ok
+     |}.
+
+End ListInst.
