CheckArith/Builtins.v
@@ -1,0 +1,234 @@
+From Coq Require Import Arith ZArith Eqdep_dec String.
+
+From Vyper Require Import Config NaryFun.
+From Vyper Require Import L10.Base CheckedArith UInt256.
+
+(** Assert that the given builtin only computes the given pure unary function. *)
+Definition BuiltinIsUnop {C: VyperConfig} (f: builtin) (unop: uint256 -> uint256)
+:= match projT1 f as arity return _ = arity -> _ with
+   | 1 => fun E => forall (w: world_state) (a: uint256),
+                     nary_call_1 (projT2 f w) E a = (w, ExprSuccess (unop a))
+   | _ => fun _ => False
+   end eq_refl.
+
+(** If a builtin is an unop, then its arity is 1. *)
+Lemma builtin_is_unop_arity {C: VyperConfig} (f: builtin) (unop: uint256 -> uint256)
+                            (Ok: BuiltinIsUnop f unop):
+  projT1 f = 1.
+Proof.
+unfold BuiltinIsUnop in Ok.
+remember (fun E : projT1 f = 1 =>
+             forall (w : world_state) (a : uint256),
+             nary_call_1 (projT2 f w) E a = (w, ExprSuccess (unop a))) as foo.
+clear Heqfoo.
+destruct (projT1 f) as [|n]; try contradiction.
+now destruct n.
+Qed.
+
+(** [nary_call] works as it should on builtins approved by BuiltinIsUnop. *)
+Lemma builtin_is_unop_call {C: VyperConfig} (f: builtin) (unop: uint256 -> uint256)
+                           (Ok: BuiltinIsUnop f unop)
+                           (w: world_state)
+                           (a: uint256)
+                           (ArityOk: projT1 f <= 1):
+  nary_call (projT2 f w) (a :: nil) ArityOk = (w, ExprSuccess (unop a), nil).
+Proof.
+assert (Arity1 := builtin_is_unop_arity f unop Ok).
+unfold BuiltinIsUnop in Ok.
+remember (fun E : projT1 f = 1 =>
+                 forall (w : world_state) (a: uint256),
+                 nary_call_1 (projT2 f w) E a = (w, ExprSuccess (unop a))) as Good.
+enough (G: Good Arity1).
+{
+  clear Ok. subst.
+  rewrite nary_call_1_ok with (E := Arity1).
+  f_equal. apply G.
+}
+clear HeqGood.
+destruct (projT1 f) as [|n]; try contradiction.
+destruct n; try contradiction.
+assert (R: Arity1 = eq_refl). { apply eq_proofs_unicity. decide equality. }
+rewrite R. assumption.
+Qed.
+
+Lemma builtin_is_unop_ok {C: VyperConfig} (f: builtin) (unop: uint256 -> uint256)
+                         (Ok: BuiltinIsUnop f unop)
+                         (w: world_state)
+                         (a: uint256)
+                         (LengthOk: (projT1 f =? Datatypes.length (a :: nil)) = true):
+  call_builtin (a :: nil) LengthOk (projT2 f w) = (w, ExprSuccess (unop a)).
+Proof.
+unfold call_builtin.
+now rewrite (builtin_is_unop_call f unop Ok w a).
+Qed.
+
+(** Assert that the given builtin only computes the given pure binary function. *)
+Definition BuiltinIsBinop {C: VyperConfig} (f: builtin) (binop: uint256 -> uint256 -> uint256)
+:= match projT1 f as arity return _ = arity -> _ with
+   | 2 => fun E => forall (w: world_state) (a b: uint256),
+                     nary_call_2 (projT2 f w) E a b = (w, ExprSuccess (binop a b))
+   | _ => fun _ => False
+   end eq_refl.
+
+(** If a builtin is an unop, then its arity is 2. *)
+Lemma builtin_is_binop_arity {C: VyperConfig} (f: builtin) (binop: uint256 -> uint256 -> uint256)
+                             (Ok: BuiltinIsBinop f binop):
+  projT1 f = 2.
+Proof.
+unfold BuiltinIsBinop in Ok.
+remember (fun E : projT1 f = 2 =>
+                 forall (w : world_state) (a b : uint256),
+                 nary_call_2 (projT2 f w) E a b = (w, ExprSuccess (binop a b))) as foo.
+clear Heqfoo.
+destruct (projT1 f) as [|n]; try contradiction.
+destruct n; try contradiction.
+now destruct n.
+Qed.
+
+(** [nary_call] works as it should on builtins approved by BuiltinIsBinop. *)
+Lemma builtin_is_binop_call {C: VyperConfig} (f: builtin) (binop: uint256 -> uint256 -> uint256)
+                            (Ok: BuiltinIsBinop f binop)
+                            (w: world_state)
+                            (a b: uint256)
+                            (ArityOk: projT1 f <= 2):
+  nary_call (projT2 f w) (a :: b :: nil) ArityOk = (w, ExprSuccess (binop a b), nil).
+Proof.
+assert (Arity2 := builtin_is_binop_arity f binop Ok).
+unfold BuiltinIsBinop in Ok.
+remember (fun E : projT1 f = 2 =>
+                 forall (w : world_state) (a b : uint256),
+                 nary_call_2 (projT2 f w) E a b = (w, ExprSuccess (binop a b))) as Good.
+enough (G: Good Arity2).
+{
+  clear Ok. subst.
+  rewrite nary_call_2_ok with (E := Arity2).
+  f_equal. apply G.
+}
+clear HeqGood.
+destruct (projT1 f) as [|n]; try contradiction.
+destruct n; try contradiction.
+destruct n; try contradiction.
+assert (R: Arity2 = eq_refl). { apply eq_proofs_unicity. decide equality. }
+rewrite R. assumption.
+Qed.
+
+Lemma builtin_is_binop_ok {C: VyperConfig} (f: builtin) (binop: uint256 -> uint256 -> uint256)
+                          (Ok: BuiltinIsBinop f binop)
+                          (w: world_state)
+                          (a b: uint256)
+                          (LengthOk: (projT1 f =? List.length (a :: b :: nil)) = true):
+  call_builtin (a :: b :: nil) LengthOk (projT2 f w) = (w, ExprSuccess (binop a b)).
+Proof.
+unfold call_builtin.
+now rewrite (builtin_is_binop_call f binop Ok w a).
+Qed.
+
+Definition builtin_of_unop {C: VyperConfig} (f: uint256 -> uint256)
+: builtin
+:= existT _ 1 (fun w =>
+                (fun a: uint256 => (w, ExprSuccess (f a))): nary_fun _ 1 _).
+
+Lemma builtin_of_unop_ok {C: VyperConfig} (f: uint256 -> uint256):
+  BuiltinIsUnop (builtin_of_unop f) f.
+Proof. easy. Qed.
+
+Definition builtin_of_binop {C: VyperConfig} (f: uint256 -> uint256 -> uint256)
+: builtin
+:= existT _ 2 (fun w =>
+                (fun (a b: uint256) => (w, ExprSuccess (f a b))): nary_fun _ 2 _).
+
+Lemma builtin_of_binop_ok {C: VyperConfig} (f: uint256 -> uint256 -> uint256):
+  BuiltinIsBinop (builtin_of_binop f) f.
+Proof. easy. Qed.
+
+
+(******************************************)
+(* Builtins for uint256 modulo arithmetic *)
+(******************************************)
+
+Definition builtin_uint256_add {C: VyperConfig} := builtin_of_binop uint256_add.
+Definition builtin_uint256_sub {C: VyperConfig} := builtin_of_binop uint256_sub.
+Definition builtin_uint256_mul {C: VyperConfig} := builtin_of_binop uint256_mul.
+Definition builtin_uint256_div {C: VyperConfig} := builtin_of_binop uint256_div.
+Definition builtin_uint256_mod {C: VyperConfig} := builtin_of_binop uint256_mod.
+Definition builtin_uint256_pow {C: VyperConfig} := builtin_of_binop uint256_pow.
+Definition builtin_uint256_shl {C: VyperConfig} := builtin_of_binop uint256_shl.
+Definition builtin_uint256_shr {C: VyperConfig} := builtin_of_binop uint256_shr.
+
+(*****************)
+(* Builtin names *)
+(*****************)
+
+Record builtin_names_config := { builtin_name_uint256_add: string
+                               ; builtin_name_uint256_sub: string
+                               ; builtin_name_uint256_mul: string
+                               ; builtin_name_uint256_div: string
+                               ; builtin_name_uint256_mod: string
+                               ; builtin_name_uint256_pow: string
+                               ; builtin_name_uint256_not: string
+                               ; builtin_name_uint256_iszero: string
+                               ; builtin_name_uint256_and: string
+                               ; builtin_name_uint256_or: string
+                               ; builtin_name_uint256_xor: string
+                               ; builtin_name_uint256_lt: string
+                               ; builtin_name_uint256_eq: string
+                               ; builtin_name_uint256_shl: string
+                               ; builtin_name_uint256_shr: string
+                               }.
+
+Definition builtin_names_std
+: builtin_names_config
+:= {| builtin_name_uint256_add    := "uint256_add"
+    ; builtin_name_uint256_sub    := "uint256_sub"
+    ; builtin_name_uint256_mul    := "uint256_mul"
+    ; builtin_name_uint256_div    := "uint256_div"
+    ; builtin_name_uint256_mod    := "uint256_mod"
+    ; builtin_name_uint256_pow    := "uint256_pow"
+    ; builtin_name_uint256_not    := "uint256_not"
+    ; builtin_name_uint256_iszero := "uint256_iszero"
+    ; builtin_name_uint256_and    := "uint256_and"
+    ; builtin_name_uint256_or     := "uint256_or"
+    ; builtin_name_uint256_xor    := "uint256_xor"
+    ; builtin_name_uint256_lt     := "uint256_lt"
+    ; builtin_name_uint256_eq     := "uint256_eq"
+    ; builtin_name_uint256_shl    := "uint256_shl"
+    ; builtin_name_uint256_shr    := "uint256_shr"
+   |}.
+
+Definition BuiltinsSupportUnop {C: VyperConfig}
+                               (builtins: string -> option builtin)
+                               (name: string)
+                               (unop: uint256 -> uint256)
+:= match builtins name with
+   | Some b => BuiltinIsUnop b unop
+   | None => False
+   end.
+
+Definition BuiltinsSupportBinop {C: VyperConfig}
+                                (builtins: string -> option builtin)
+                                (name: string)
+                                (binop: uint256 -> uint256 -> uint256)
+:= match builtins name with
+   | Some b => BuiltinIsBinop b binop
+   | None => False
+   end.
+
+
+Definition BuiltinsSupportUInt256 {C: VyperConfig}
+                                  (names: builtin_names_config)
+                                  (builtins: string -> option builtin)
+:= BuiltinsSupportBinop builtins (builtin_name_uint256_add names) uint256_add
+/\ BuiltinsSupportBinop builtins (builtin_name_uint256_sub names) uint256_sub
+/\ BuiltinsSupportBinop builtins (builtin_name_uint256_mul names) uint256_mul
+/\ BuiltinsSupportBinop builtins (builtin_name_uint256_div names) uint256_div
+/\ BuiltinsSupportBinop builtins (builtin_name_uint256_mod names) uint256_mod
+/\ BuiltinsSupportBinop builtins (builtin_name_uint256_pow names) uint256_pow
+/\ BuiltinsSupportUnop  builtins (builtin_name_uint256_not names) uint256_not
+/\ BuiltinsSupportUnop  builtins (builtin_name_uint256_iszero names) uint256_iszero
+/\ BuiltinsSupportBinop builtins (builtin_name_uint256_and names) uint256_and
+/\ BuiltinsSupportBinop builtins (builtin_name_uint256_or  names) uint256_or
+/\ BuiltinsSupportBinop builtins (builtin_name_uint256_xor names) uint256_xor
+/\ BuiltinsSupportBinop builtins (builtin_name_uint256_lt  names) uint256_lt
+/\ BuiltinsSupportBinop builtins (builtin_name_uint256_eq  names) uint256_eq
+/\ BuiltinsSupportBinop builtins (builtin_name_uint256_shl names) uint256_shl
+/\ BuiltinsSupportBinop builtins (builtin_name_uint256_shr names) uint256_shr.
