CheckArith/Translate.v
@@ -1,0 +1,442 @@
+From Coq Require Import NArith ZArith Lia String HexString.
+
+From Vyper Require Import Config Calldag.
+From Vyper.L30 Require Import AST Callset Descend VarCap.
+
+From Vyper.CheckArith Require Import Builtins CheckedArith.
+
+Definition arithmetic_error
+:= Z.of_N
+     (List.fold_left (fun x y => N.lor (N.shiftl x 8) y)
+       (List.map Ascii.N_of_ascii (list_ascii_of_string "arithmetic error"))
+       0%N).
+
+Example hex_arithmetic_error:
+  HexString.of_Z arithmetic_error = "0x61726974686d65746963206572726f72"%string.
+                                    (*  a r i t h m e t i c   e r r o r *)
+Proof. trivial. Qed.
+
+(** AST for [dst = "arithmetic error"; raise dst] *)
+Definition ast_raise_arithmetic_error {C: VyperConfig} (dst: N)
+: stmt
+:= Semicolon (SmallStmt (Const dst (uint256_of_Z arithmetic_error)))
+             (SmallStmt (Raise dst)).
+
+(** AST for [scratch[0] = a; scratch[1] = b] *)
+Definition ast_pair_to_scratch {C: VyperConfig} (a b: N) (scratch: N)
+: stmt
+:= Semicolon (SmallStmt (Copy scratch a))
+             (SmallStmt (Copy (N.succ scratch) b)).
+
+Definition translate_small_stmt {C: VyperConfig} (B: builtin_names_config)
+                                (scratch: N)
+                                (ss: small_stmt)
+: stmt
+:= match ss with
+   | UnOp op dst src =>
+      match op with
+      | L10.AST.BitwiseNot =>
+          SmallStmt (BuiltinCall dst (builtin_name_uint256_not B) src 1%N)
+      | L10.AST.LogicalNot =>
+          SmallStmt (BuiltinCall dst (builtin_name_uint256_iszero B) src 1%N)
+      | L10.AST.Neg =>
+          (* if src:
+               scratch = "arithmetic error"
+               raise scratch
+             else:
+               dst = 0
+           *)
+          (IfElseStmt src
+            (ast_raise_arithmetic_error scratch)
+            (SmallStmt (Const dst zero256)))
+      end
+   | BinOp op dst a b NEpow =>
+      match op as op' return op = op' -> _ with
+      | L10.AST.BitwiseAnd => fun _ =>
+          Semicolon (ast_pair_to_scratch a b scratch)
+            (SmallStmt (BuiltinCall dst (builtin_name_uint256_and B) scratch 2%N))
+      | L10.AST.BitwiseOr => fun _ =>
+          Semicolon (ast_pair_to_scratch a b scratch)
+                    (SmallStmt (BuiltinCall dst (builtin_name_uint256_or B) scratch 2%N))
+      | L10.AST.BitwiseXor => fun _ =>
+          Semicolon (ast_pair_to_scratch a b scratch)
+                    (SmallStmt (BuiltinCall dst (builtin_name_uint256_xor B) scratch 2%N))
+      | L10.AST.Lt => fun _ =>
+          Semicolon (ast_pair_to_scratch a b scratch)
+                    (SmallStmt (BuiltinCall dst (builtin_name_uint256_lt B) scratch 2%N))
+      | L10.AST.Gt => fun _ =>
+          Semicolon (ast_pair_to_scratch b a scratch)
+                    (SmallStmt (BuiltinCall dst (builtin_name_uint256_lt B) scratch 2%N))
+      | L10.AST.Eq => fun _ =>
+          Semicolon (ast_pair_to_scratch a b scratch)
+                    (SmallStmt (BuiltinCall dst (builtin_name_uint256_eq B) scratch 2%N))
+      | L10.AST.Ne => fun _ =>
+          Semicolon 
+            (ast_pair_to_scratch a b scratch)
+            (Semicolon
+              (SmallStmt (BuiltinCall dst (builtin_name_uint256_eq B) scratch 2%N))
+              (SmallStmt (BuiltinCall dst (builtin_name_uint256_iszero B) dst 1%N)))
+      | L10.AST.Ge => fun _ =>
+          Semicolon 
+            (ast_pair_to_scratch a b scratch)
+            (Semicolon
+              (SmallStmt (BuiltinCall dst (builtin_name_uint256_lt B) scratch 2%N))
+              (SmallStmt (BuiltinCall dst (builtin_name_uint256_iszero B) dst 1%N)))
+      | L10.AST.Le => fun _ =>
+          Semicolon 
+            (ast_pair_to_scratch b a scratch)
+            (Semicolon
+              (SmallStmt (BuiltinCall dst (builtin_name_uint256_lt B) scratch 2%N))
+              (SmallStmt (BuiltinCall dst (builtin_name_uint256_iszero B) dst 1%N)))
+      | L10.AST.Add => fun _ =>
+          (*
+            scratch[0] = a                                     # a
+            scratch[1] = b                                     # a           b
+            scratch[1] = builtin("uint256_add", scratch, 2)    # a           a + b
+            scratch[0] = builtin("uint256_lt", scratch, 2)     # a < a + b   a + b
+            if scratch[0]:
+              dst = scratch[1]
+            else:
+              raise "arithmetic error"
+          *)
+          Semicolon
+            (ast_pair_to_scratch a b scratch)
+            (Semicolon
+              (Semicolon
+                (SmallStmt (BuiltinCall (N.succ scratch)
+                                        (builtin_name_uint256_add B)
+                                        scratch 2%N))
+                (SmallStmt (BuiltinCall scratch
+                                        (builtin_name_uint256_lt B)
+                                        scratch 2%N)))
+              (IfElseStmt scratch
+                (SmallStmt (Copy dst (N.succ scratch)))
+                (ast_raise_arithmetic_error scratch)))
+      | L10.AST.Sub => fun _ =>
+          (*
+             scratch0 = a
+             scratch1 = b
+             dst = builtin("uint256_lt", scratch, 2)
+             if dst:
+               raise "arithmetic error"
+             else:
+               dst = builtin("uint256_sub", scratch, 2)
+          *)
+          Semicolon
+            (ast_pair_to_scratch a b scratch)
+            (Semicolon
+              (SmallStmt (BuiltinCall dst (builtin_name_uint256_lt B) scratch 2%N))
+              (IfElseStmt dst
+                (ast_raise_arithmetic_error scratch)
+                (SmallStmt (BuiltinCall dst (builtin_name_uint256_sub B) scratch 2))))
+      | L10.AST.Mul => fun _ =>
+          (*
+             if a:
+               scratch1 = a                                    #       a
+               scratch2 = b                                    #       a         b
+               scratch0 = builtin("uint256_mul", scratch1, 2)  # a*b   a         b
+               scratch1 = builtin("uint256_div", scratch0, 2)  # a*b   a*b/a     b
+               scratch1 = builtin("uint256_eq",  scratch1, 2)  # a*b   a*b/a==b  b
+               if scratch1:
+                 dst = scratch0
+               else:
+                 raise "arithmetic error"
+             else:
+               dst = 0
+          *)
+          IfElseStmt a
+            (Semicolon
+               (ast_pair_to_scratch a b (N.succ scratch))
+               (Semicolon
+                 (Semicolon
+                   (SmallStmt (BuiltinCall scratch (builtin_name_uint256_mul B)
+                                           (N.succ scratch) 2%N))
+                   (Semicolon
+                     (SmallStmt (BuiltinCall (N.succ scratch) (builtin_name_uint256_div B)
+                                             scratch 2%N))
+                     (SmallStmt (BuiltinCall (N.succ scratch) (builtin_name_uint256_eq B)
+                                             (N.succ scratch) 2%N))))
+                 (IfElseStmt (N.succ scratch)
+                   (SmallStmt (Copy dst scratch))
+                   (ast_raise_arithmetic_error scratch))))
+            (SmallStmt (Const dst zero256))
+      | L10.AST.Quot => fun _ =>
+          (*
+             if b:
+               scratch[0] = a
+               scratch[1] = b
+               dst = builtin("uint256_div",  scratch1, 2)
+             else
+               raise "arithmetic error"
+          *)
+          IfElseStmt b
+            (Semicolon
+              (ast_pair_to_scratch a b scratch)
+              (SmallStmt (BuiltinCall dst (builtin_name_uint256_div B) scratch 2%N)))
+            (ast_raise_arithmetic_error scratch)
+      | L10.AST.Mod => fun _ =>
+          (*
+             if b:
+               scratch[0] = a
+               scratch[1] = b
+               dst = builtin("uint256_mod",  scratch1, 2)
+             else
+               raise "arithmetic error"
+          *)
+          IfElseStmt b
+                (Semicolon
+                  (ast_pair_to_scratch a b scratch)
+                  (SmallStmt (BuiltinCall dst (builtin_name_uint256_mod B) scratch 2%N)))
+                (ast_raise_arithmetic_error scratch)
+      | L10.AST.ShiftRight => fun _ =>
+          Semicolon
+                (ast_pair_to_scratch a b scratch)
+                (SmallStmt (BuiltinCall dst (builtin_name_uint256_shr B) scratch 2%N))
+      | L10.AST.ShiftLeft => fun _ =>
+          (*
+             scratch0 = a                                   #    a
+             scratch1 = b                                   #    a            b
+             scratch0 = builtin("uint256_shl", scratch, 2)  #    a<<b         b
+             scratch1 = builtin("uint256_shr", scratch, 2)  #    a<<b         (a<<b)>>b
+             dst = scratch0
+             scratch0 = a                                   #    a            (a<<b)>>b
+             scratch0 = builtin("uint256_eq", scratch, 2)   #    a==(a<<b)>>b (a<<b)>>b
+             if scratch0:
+               pass
+             else:
+               raise "arithmetic error"
+          *)
+          Semicolon
+             (ast_pair_to_scratch a b (N.succ scratch))
+             (Semicolon
+               (SmallStmt (BuiltinCall scratch (builtin_name_uint256_shl B) scratch 2%N))
+               (Semicolon
+                 (SmallStmt (BuiltinCall (N.succ scratch) (builtin_name_uint256_shr B)
+                                         scratch 2%N))
+                 (Semicolon
+                   (SmallStmt (Copy dst scratch))
+                   (Semicolon
+                     (SmallStmt (Copy scratch a))
+                     (Semicolon
+                       (SmallStmt (BuiltinCall scratch (builtin_name_uint256_eq B)
+                                               scratch 2%N))
+                       (IfElseStmt scratch
+                         (SmallStmt Pass)
+                         (ast_raise_arithmetic_error scratch)))))))
+      | L10.AST.Pow => fun E => False_rect _ (NEpow E)
+      end eq_refl
+   | PowConstBase dst base exp =>
+       let zbase := Z_of_uint256 base in
+       if (zbase =? 0)%Z
+         then (* iszero(exp) *)
+              SmallStmt (BuiltinCall dst (builtin_name_uint256_iszero B) exp 1%N)
+         else
+           if (zbase =? 1)%Z
+             then SmallStmt (Const dst one256) (* 1 *)
+             else
+               if (zbase =? 2)%Z
+                 then (* scratch1 = exp
+                         scratch2 = 256
+                         scratch2 = builtin("uint256_lt", scratch1, 2)
+                         if scratch2:
+                           scratch0 = 1
+                           dst = builtin("uint256_shl", scratch0, 2)
+                         else:
+                           raise "arithmetic error"
+                      *)
+                      Semicolon
+                        (SmallStmt (Copy (N.succ scratch) exp))
+                        (Semicolon
+                          (SmallStmt (Const (scratch + 2)%N (uint256_of_Z 256%Z)))
+                          (Semicolon
+                            (SmallStmt (BuiltinCall (scratch + 2)%N
+                                                    (builtin_name_uint256_lt B)
+                                                    (N.succ scratch) 2%N))
+                            (IfElseStmt (scratch + 2)%N
+                              (Semicolon
+                                (SmallStmt (Const scratch one256))
+                                (SmallStmt (BuiltinCall dst
+                                                        (builtin_name_uint256_shl B)
+                                                        scratch 2%N)))
+                              (ast_raise_arithmetic_error scratch))))
+                 else (*
+                         scratch0 = uint256_max_power base
+                         scratch1 = exp
+                         dst = builtin("uint256_lt", scratch, 2)
+                         if dst:
+                           raise "arithmetic error"
+                         else:
+                           scratch0 = base
+                           dst = builtin("uint256_pow", scratch, 2)
+                      *)
+                      Semicolon
+                        (SmallStmt (Const scratch
+                                     (uint256_of_Z (uint256_max_power zbase))))
+                        (Semicolon
+                          (SmallStmt (Copy (N.succ scratch) exp))
+                          (Semicolon
+                            (SmallStmt (BuiltinCall dst (builtin_name_uint256_lt B)
+                                                    scratch 2))
+                            (IfElseStmt dst
+                              (ast_raise_arithmetic_error scratch)
+                              (Semicolon
+                                (SmallStmt (Const scratch base))
+                                (SmallStmt (BuiltinCall dst (builtin_name_uint256_pow B)
+                                                        scratch 2))))))
+   | PowConstExp dst base exp =>
+      let zexp := Z_of_uint256 exp in
+      if (zexp =? 0)%Z
+        then SmallStmt (Const dst one256) (* 1 *)
+        else
+          if (zexp =? 1)%Z
+            then (* we do actually have to compute base ** 1 to canonicalize uint256 *)
+              Semicolon
+                (SmallStmt (Copy scratch base))
+                (Semicolon
+                  (SmallStmt (Const (N.succ scratch) one256))
+                  (SmallStmt (BuiltinCall dst (builtin_name_uint256_pow B)
+                                          scratch 2)))
+            else (*
+                   scratch0 = base
+                   scratch1 = uint256_max_base zexp + 1
+                   dst = builtin("uint256_lt", scratch, 2)
+                   if dst:
+                     scratch0 = exp
+                     dst = builtin("uint256_pow", scratch, 2)
+                   else:
+                     raise "arithmetic error"
+                 *)
+             Semicolon
+               (SmallStmt (Copy scratch base))
+               (Semicolon
+                 (SmallStmt (Const (N.succ scratch)
+                                   (uint256_of_Z (Z.succ (uint256_max_base zexp)))))
+                 (Semicolon
+                   (SmallStmt (BuiltinCall dst (builtin_name_uint256_lt B)
+                                           scratch 2))
+                   (IfElseStmt dst
+                     (Semicolon
+                       (SmallStmt (Const scratch exp))
+                       (SmallStmt (BuiltinCall dst (builtin_name_uint256_pow B)
+                                               scratch 2)))
+                     (ast_raise_arithmetic_error scratch))))
+   | _ => SmallStmt ss
+   end.
+
+Fixpoint translate_stmt {C: VyperConfig} (B: builtin_names_config)
+                        (scratch: N)
+                        (s: stmt)
+{struct s}
+: stmt
+:= match s with
+   | SmallStmt ss => translate_small_stmt B scratch ss
+   | IfElseStmt cond yes no => IfElseStmt cond (translate_stmt B scratch yes)
+                                               (translate_stmt B scratch no)
+   | Loop var count body => Loop var count (translate_stmt B scratch body)
+   | Semicolon a b => Semicolon (translate_stmt B scratch a)
+                                (translate_stmt B scratch b)
+   end.
+
+Definition translate_decl {C: VyperConfig} (B: builtin_names_config)
+                          (scratch: N)
+                          (d: decl)
+: decl
+:= match d with
+   | StorageVarDecl var => d
+   | FunDecl name arity body => FunDecl name arity (translate_stmt B scratch body)
+   end.
+
+Ltac rr := cbn; trivial;
+           repeat rewrite FSet.union_ok;
+           repeat rewrite FSet.empty_ok;
+           trivial.
+
+Lemma callset_translate_small_stmt {C: VyperConfig}
+                                   (B: builtin_names_config)
+                                   (scratch: N)
+                                   (ss: small_stmt)
+                                   (x: string):
+  let _ := string_set_impl in
+  FSet.has (stmt_callset (translate_small_stmt B scratch ss)) x
+   =
+  FSet.has (small_stmt_callset ss) x.
+Proof.
+cbn.
+destruct ss; simpl; trivial. (* cbn hangs *)
+{ (* UnOp *) destruct op; rr. }
+{ (* PowConstBase *)
+  destruct Z.eqb. { easy. }
+  destruct Z.eqb. { easy. }
+  destruct Z.eqb; rr.
+}
+{ (* PowConstExp *)
+  destruct Z.eqb. { easy. }
+  destruct Z.eqb; cbn; rr.
+}
+(* Binop *)
+destruct op; simpl; rr.
+contradiction.
+Qed.
+
+Lemma callset_translate_stmt {C: VyperConfig}
+                             (B: builtin_names_config)
+                             (scratch: N)
+                             (s: stmt)
+                             (x: string):
+  let _ := string_set_impl in
+  FSet.has (stmt_callset (translate_stmt B scratch s)) x
+   =
+  FSet.has (stmt_callset s) x.
+Proof.
+cbn.
+induction s; cbn; try assumption.
+{ (* SmallStmt *) apply callset_translate_small_stmt. }
+1-2: repeat rewrite FSet.union_ok;
+     rewrite IHs1; rewrite IHs2;
+     trivial.
+Qed.
+
+Lemma callset_translate_decl {C: VyperConfig}
+                             (B: builtin_names_config)
+                             (scratch: N)
+                             (d: decl)
+                             (x: string):
+  let _ := string_set_impl in
+  FSet.has (decl_callset (translate_decl B scratch d)) x
+   =
+  FSet.has (decl_callset d) x.
+Proof.
+destruct d; cbn. { easy. }
+apply callset_translate_stmt.
+Qed.
+
+Local Lemma translate_calldag_helper {C: VyperConfig}
+                                     (B: builtin_names_config)
+                                     (scratch: N)
+                                     (cd: calldag):
+  let H := string_set_impl in
+  forall d: decl,
+    FSet.is_subset (decl_callset (translate_decl B scratch d)) (decl_callset d) = true.
+Proof.
+cbn. intro.
+apply FSet.is_subset_equal.
+apply FSet.equal_ok.
+apply callset_translate_decl.
+Qed.
+
+Definition translate_calldag {C: VyperConfig}
+                             (B: builtin_names_config)
+                             (scratch: N)
+                             (cd: calldag)
+:= calldag_map (translate_decl B scratch)
+               (translate_calldag_helper B scratch cd)
+               cd.
+
+Definition translate_fun_ctx {C: VyperConfig}
+                             (B: builtin_names_config)
+                             (scratch: N)
+                             {bound: nat}
+                             {cd: calldag}
+                             (fc: fun_ctx cd bound)
+: fun_ctx (calldag_map (translate_decl B scratch) (translate_calldag_helper B scratch cd) cd) bound
+:= fun_ctx_map (translate_decl B scratch) _ cd fc.
