Extract.v
@@ -5,6 +5,7 @@ From Vyper Require L10.ToString L30.AST.
 
 From Coq Require Import ZArith.
 Definition z_eqb := Z.eqb.
+Definition l10_neg := L10.AST.Neg.
 Definition l10_decls_to_string {C: VyperConfig} := L10.ToString.string_of_decls.
 Definition l30_decls_to_string {C: VyperConfig} := L30.AST.string_of_decls.
 
@@ -21,5 +22,6 @@ Extraction "haskell/Extracted.hs"
   compile
   uint256_of_Z
   sample_config
+  l10_neg
   l10_decls_to_string
   l30_decls_to_string.
