Hash/Keccak.v
@@ -1,0 +1,419 @@
+(**
+  This is Keccak-256 and SHA3-256 ported from Go's 
+    golang.org/x/crypto/sha3
+ *)
+
+From Coq Require Import List.
+From Coq Require HexString.
+From Coq Require Import String.
+From Coq Require Import NArith ZArith Lia.
+From Coq Require Import Int63.
+
+From Vyper Require UInt64 Tuplevector.
+From Vyper Require Import Nibble.
+
+Local Open Scope string_scope.
+
+Definition rc_hex: list string
+:= "0x0000000000000001"
+:: "0x0000000000008082"
+:: "0x800000000000808A"
+:: "0x8000000080008000"
+:: "0x000000000000808B"
+:: "0x0000000080000001"
+:: "0x8000000080008081"
+:: "0x8000000000008009"
+:: "0x000000000000008A"
+:: "0x0000000000000088"
+:: "0x0000000080008009"
+:: "0x000000008000000A"
+:: "0x000000008000808B"
+:: "0x800000000000008B"
+:: "0x8000000000008089"
+:: "0x8000000000008003"
+:: "0x8000000000008002"
+:: "0x8000000000000080"
+:: "0x000000000000800A"
+:: "0x800000008000000A"
+:: "0x8000000080008081"
+:: "0x8000000000008080"
+:: "0x0000000080000001"
+:: "0x8000000080008008"
+:: nil.
+
+Definition rc := map UInt64.uint64_of_Z_mod (map HexString.to_Z rc_hex).
+Lemma rc_ok:
+  map UInt64.Z_of_uint64 rc = map HexString.to_Z rc_hex.
+Proof. trivial. Qed.
+
+Definition rc_quads_backwards := Tuplevector.gather rc 6 4 eq_refl.
+
+Inductive vec25 (T: Type)
+:= Vec25 (a0  a1  a2  a3  a4
+          a5  a6  a7  a8  a9
+          a10 a11 a12 a13 a14
+          a15 a16 a17 a18 a19
+          a20 a21 a22 a23 a24: T).
+Arguments Vec25 {_}.
+
+Definition vec25_fill {T: Type} (x: T)
+:= Vec25 x x x x x
+         x x x x x
+         x x x x x
+         x x x x x
+         x x x x x.
+
+Definition uint64 := UInt64.uint64.
+
+Definition vec25_zeros := vec25_fill (UInt64.uint64_0).
+
+Section Permutation.
+
+Local Notation "x ^ y"  := (UInt64.bitwise_xor x y).
+
+Definition vec25_xor_tuple17_backwards (a: vec25 uint64) (b: Tuplevector.t uint64 17)
+:= match a with
+   | Vec25 a0  a1  a2  a3  a4
+           a5  a6  a7  a8  a9
+          a10 a11 a12 a13 a14
+          a15 a16 a17 a18 a19
+          a20 a21 a22 a23 a24 =>
+      match b with
+      | (b16, b15, b14, b13, b12, b11, b10, b9, b8, b7, b6, b5, b4, b3, b2, b1, b0) =>
+             Vec25 ( a0 ^  b0)  (a1 ^  b1)  (a2 ^  b2)  (a3 ^  b3)  (a4 ^  b4)
+                   ( a5 ^  b5)  (a6 ^  b6)  (a7 ^  b7)  (a8 ^  b8)  (a9 ^  b9)
+                   (a10 ^ b10) (a11 ^ b11) (a12 ^ b12) (a13 ^ b13) (a14 ^ b14)
+                   (a15 ^ b15) (a16 ^ b16)  a17         a18         a19
+                    a20         a21         a22         a23         a24
+      end
+   end.
+
+Local Notation "x << y" := (UInt64.shl_uint63 x y).
+Local Notation "x >> y" := (UInt64.shr_uint63 x y).
+Local Notation "x | y"  := (UInt64.bitwise_or x y)  (at level 30). (* dangerous! messes up match! *)
+Local Notation "x & y"  := (UInt64.bitwise_and x y) (at level 30).
+Local Notation "~ x"  := (UInt64.bitwise_not x).
+
+Definition rot x k := ((x << k) | (x >> (64 - k)%int63)).
+
+Definition round (rc: uint64) (a: vec25 uint64) (b: vec25 uint64)
+: vec25 uint64
+:= match a, b with
+   | Vec25 a0  a1  a2  a3  a4
+           a5  a6  a7  a8  a9
+           a10 a11 a12 a13 a14
+           a15 a16 a17 a18 a19
+           a20 a21 a22 a23 a24,
+     Vec25 b0  b1  b2  b3  b4
+           b5  b6  b7  b8  b9
+           b10 b11 b12 b13 b14
+           b15 b16 b17 b18 b19
+           b20 b21 b22 b23 b24 =>
+ 
+      let bc0 := a0 ^ a5 ^ a10 ^ a15 ^ a20 in
+      let bc1 := a1 ^ a6 ^ a11 ^ a16 ^ a21 in
+      let bc2 := a2 ^ a7 ^ a12 ^ a17 ^ a22 in
+      let bc3 := a3 ^ a8 ^ a13 ^ a18 ^ a23 in
+      let bc4 := a4 ^ a9 ^ a14 ^ a19 ^ a24 in
+
+      let d0 := bc4 ^ rot bc1 1%int63 in
+      let d1 := bc0 ^ rot bc2 1%int63 in
+      let d2 := bc1 ^ rot bc3 1%int63 in
+      let d3 := bc2 ^ rot bc4 1%int63 in
+      let d4 := bc3 ^ rot bc0 1%int63 in
+
+      let p0 := b0 ^ d0 in
+      let p1 := rot (b1 ^ d1) 44%int63 in
+      let p2 := rot (b2 ^ d2) 43%int63 in
+      let p3 := rot (b3 ^ d3) 21%int63 in
+      let p4 := rot (b4 ^ d4) 14%int63 in
+
+      let z0  := p0 ^ (p2 & ~ p1) ^ rc in
+      let z1  := p1 ^ (p3 & ~ p2) in
+      let z2  := p2 ^ (p4 & ~ p3) in
+      let z3  := p3 ^ (p0 & ~ p4) in
+      let z4  := p4 ^ (p1 & ~ p0) in
+
+      let q2 := rot (b5 ^ d0)  3%int63 in
+      let q3 := rot (b6 ^ d1) 45%int63 in
+      let q4 := rot (b7 ^ d2) 61%int63 in
+      let q0 := rot (b8 ^ d3) 28%int63 in
+      let q1 := rot (b9 ^ d4) 20%int63 in
+
+      let z5  := q0 ^ (q2 & ~ q1) in
+      let z6  := q1 ^ (q3 & ~ q2) in
+      let z7  := q2 ^ (q4 & ~ q3) in
+      let z8  := q3 ^ (q0 & ~ q4) in
+      let z9  := q4 ^ (q1 & ~ q0) in
+
+      let r4 := rot (b10 ^ d0) 18%int63 in
+      let r0 := rot (b11 ^ d1)  1%int63 in
+      let r1 := rot (b12 ^ d2)  6%int63 in
+      let r2 := rot (b13 ^ d3) 25%int63 in
+      let r3 := rot (b14 ^ d4)  8%int63 in
+
+      let z10 := r0 ^ (r2 & ~ r1) in
+      let z11 := r1 ^ (r3 & ~ r2) in
+      let z12 := r2 ^ (r4 & ~ r3) in
+      let z13 := r3 ^ (r0 & ~ r4) in
+      let z14 := r4 ^ (r1 & ~ r0) in
+
+      let s1 := rot (b15 ^ d0) 36%int63 in
+      let s2 := rot (b16 ^ d1) 10%int63 in
+      let s3 := rot (b17 ^ d2) 15%int63 in
+      let s4 := rot (b18 ^ d3) 56%int63 in
+      let s0 := rot (b19 ^ d4) 27%int63 in
+
+      let z15 := s0 ^ (s2 & ~ s1) in
+      let z16 := s1 ^ (s3 & ~ s2) in
+      let z17 := s2 ^ (s4 & ~ s3) in
+      let z18 := s3 ^ (s0 & ~ s4) in
+      let z19 := s4 ^ (s1 & ~ s0) in
+
+      let t3 := rot (b20 ^ d0) 41%int63 in
+      let t4 := rot (b21 ^ d1)  2%int63 in
+      let t0 := rot (b22 ^ d2) 62%int63 in
+      let t1 := rot (b23 ^ d3) 55%int63 in
+      let t2 := rot (b24 ^ d4) 39%int63 in
+
+      let z20 := t0 ^ (t2 & ~ t1) in
+      let z21 := t1 ^ (t3 & ~ t2) in
+      let z22 := t2 ^ (t4 & ~ t3) in
+      let z23 := t3 ^ (t0 & ~ t4) in
+      let z24 := t4 ^ (t1 & ~ t0) in
+
+      Vec25 z0  z1  z2  z3  z4
+            z5  z6  z7  z8  z9
+            z10 z11 z12 z13 z14
+            z15 z16 z17 z18 z19
+            z20 z21 z22 z23 z24
+   end.
+
+Definition permute1 {T} (a: vec25 T)
+:= match a with
+   | Vec25 a0  a1  a2  a3  a4
+           a5  a6  a7  a8  a9
+           a10 a11 a12 a13 a14
+           a15 a16 a17 a18 a19
+           a20 a21 a22 a23 a24 =>
+     Vec25 a0  a11 a22 a8  a19
+           a15 a1  a12 a23 a9
+           a5  a16 a2  a13 a24
+           a20 a6  a17 a3  a14
+           a10 a21 a7  a18 a4
+   end.
+Definition permute2 {T} (a: vec25 T)
+:= match a with
+   | Vec25 a0  a1  a2  a3  a4
+           a5  a6  a7  a8  a9
+           a10 a11 a12 a13 a14
+           a15 a16 a17 a18 a19
+           a20 a21 a22 a23 a24 =>
+     Vec25 a0  a16 a7  a23 a14
+           a20 a11 a2  a18 a9
+           a15 a6  a22 a13 a4
+           a10 a1  a17 a8  a24
+           a5  a21 a12 a3  a19
+   end.
+Definition permute3 {T} (a: vec25 T)
+:= match a with
+   | Vec25 a0  a1  a2  a3  a4
+           a5  a6  a7  a8  a9
+           a10 a11 a12 a13 a14
+           a15 a16 a17 a18 a19
+           a20 a21 a22 a23 a24 =>
+     Vec25 a0  a6  a12 a18 a24
+           a10 a16 a22 a3  a9
+           a20 a1  a7  a13 a19
+           a5  a11 a17 a23 a4
+           a15 a21 a2  a8  a14
+   end.
+Lemma permute1_of_permute3 {T} (a: vec25 T):
+  permute1 (permute3 a) = a.
+Proof. now destruct a. Qed.
+Lemma permute3_of_permute1 {T} (a: vec25 T):
+  permute3 (permute1 a) = a.
+Proof. now destruct a. Qed.
+Lemma permute2_of_permute2 {T} (a: vec25 T):
+  permute2 (permute2 a) = a.
+Proof. now destruct a. Qed.
+
+
+Definition quad_round (a: vec25 uint64) (rcs: Tuplevector.t uint64 4)
+: vec25 uint64
+:= match rcs with
+   | (rc4, rc3, rc2, rc1) =>
+        let a1 := permute1 (round rc1 a  (permute3 a))  in
+        let a2 := permute2 (round rc2 a1 (permute2 a1)) in
+        let a3 := permute3 (round rc3 a2 (permute1 a2)) in
+        round rc4 a3 a3
+   end.
+
+Definition F1600 := fold_left quad_round rc_quads_backwards.
+
+End Permutation.
+
+(* Create padding of the given length (of the padding, not of the data). *)
+Definition padding (len: positive) (start: int) (* start is 1 for Ethereum's Keccak, otherwise 6 *)
+: list byte
+:= match len with
+   | 1%positive => byte_of_int (128 lor start)%int63 :: nil
+   | _ => (byte_of_int start) :: repeat (byte_of_int 0) (N.to_nat (N.pos len - 2)) ++ 
+            byte_of_int 128 :: nil
+   end.
+
+(* The padding has the requested length *)
+Lemma padding_ok (len: positive) (start: int):
+  List.length (padding len start) = Pos.to_nat len.
+Proof.
+unfold padding.
+remember (byte_of_int start :: 
+          repeat (byte_of_int 0) (N.to_nat (N.pos len - 2)) ++
+          byte_of_int 128 ::
+          nil) as l.
+assert (cons_length: forall {T} h (t: list T), List.length (h :: t) = S (List.length t)) by easy.
+destruct len; cbn; subst;
+  repeat (rewrite List.app_length || rewrite List.repeat_length || rewrite cons_length);
+  replace (List.length (@nil byte)) with 0 by trivial; lia.
+Qed.
+
+(** Calculate the padding length given the data length. *)
+Definition padding_length (data_length: N) (rate: positive)
+: positive
+:= match (data_length mod N.pos rate)%N with
+   | 0%N => rate
+   | Npos p => rate - p
+   end.
+
+Lemma padding_length_ok (data_length: N) (rate: positive):
+  ((data_length + N.pos (padding_length data_length rate)) mod N.pos rate = 0)%N.
+Proof.
+unfold padding_length.
+remember (data_length mod N.pos rate)%N as m.
+destruct m; rewrite N.add_mod by discriminate; rewrite<- Heqm.
+{ rewrite N.add_0_l. rewrite N.mod_same by discriminate. apply N.mod_0_l. discriminate. }
+assert(L: (N.pos p < N.pos rate)%N).
+{ rewrite Heqm. apply N.mod_upper_bound. discriminate. }
+replace (N.pos (rate - p) mod N.pos rate)%N with (N.pos (rate - p)).
+2:{ symmetry. apply N.mod_small. lia. }
+replace (N.pos p + N.pos (rate - p))%N with (N.pos rate) by lia.
+apply N.mod_same. discriminate.
+Qed.
+
+Definition pad (unpadded_data: list byte) (rate: positive) (start: int)
+: list byte
+:= (unpadded_data ++ padding (padding_length (N.of_nat (List.length unpadded_data)) rate) start)%list.
+
+Lemma pad_ok_mod (data: list byte) (rate: positive) (start: int):
+  (N.of_nat (List.length (pad data rate start)) mod N.pos rate = 0)%N.
+Proof.
+unfold pad. rewrite List.app_length. rewrite Nat2N.inj_add.
+remember (List.length data) as n. rewrite padding_ok.
+rewrite positive_nat_N. rewrite padding_length_ok.
+trivial.
+Qed.
+
+Lemma pad_ok (data: list byte) (rate: positive) (start: int):
+  let d := List.length (pad data rate start) / Pos.to_nat rate in
+    List.length (pad data rate start) = d * Pos.to_nat rate.
+Proof.
+apply Nat2N.inj.
+assert (M := pad_ok_mod data rate start).
+remember (List.length  _) as len. clear Heqlen.
+match goal with |- ?lhs = ?rhs => rewrite<- (N.add_0_r rhs) end.
+rewrite<- M.
+rewrite Nat.mul_comm.
+rewrite Nat2N.inj_mul.
+rewrite Arith2.Nat2N_inj_div.
+remember (Pos.to_nat rate) as r.
+assert (R: N.pos rate = N.of_nat r).
+{ subst. symmetry. apply positive_nat_N. }
+rewrite R. rewrite R in M.
+apply N.div_mod.
+subst. assert(P := Pos2Nat.is_pos rate).
+destruct (Pos.to_nat rate).
+{ now apply Nat.lt_irrefl in P. }
+discriminate.
+Qed.
+
+Local Lemma can_gather_by_8 (n: nat):
+  n = n / 136 * 136  ->  n = (n / 136 * 17) * 8.
+Proof.
+now rewrite<- Nat.mul_assoc.
+Qed.
+
+Definition pad_by_136_and_gather_into_uint64s (data: list byte) (padding_start: int)
+:= let padded := pad data 136%positive padding_start in
+   let PadOk  := pad_ok data 136%positive padding_start in
+   List.map UInt64.uint64_of_be_bytes
+            (Tuplevector.gather padded _ 8 (can_gather_by_8 _ PadOk)).
+
+Lemma pad_by_136_and_gather_into_uint64s_length (data: list byte) (s: int):
+  List.length (pad_by_136_and_gather_into_uint64s data s) 
+   =
+  (List.length (pad data 136 s)) / 136 * 17.
+Proof.
+unfold pad_by_136_and_gather_into_uint64s.
+rewrite List.map_length.
+apply (Tuplevector.gather_length (pad data 136 s)
+             (Datatypes.length (pad data 136 s) / 136 * 17) 8
+             (can_gather_by_8 (Datatypes.length (pad data 136 s)) (pad_ok data 136 s))).
+Qed.
+
+Definition blocks (data: list byte) (padding_start: int)
+:= Tuplevector.gather (pad_by_136_and_gather_into_uint64s data padding_start)
+                      _ 17
+                      (pad_by_136_and_gather_into_uint64s_length data padding_start).
+
+Definition absorb (data: list byte) (padding_start: int)
+:= fold_left (fun state block => F1600 (vec25_xor_tuple17_backwards state block))
+             (blocks data padding_start)
+             vec25_zeros.
+
+Definition squeeze_256 (a: vec25 uint64) 
+:= match a with
+   | Vec25 a0  a1  a2  a3  _
+           _   _   _   _   _
+           _   _   _   _   _
+           _   _   _   _   _
+           _   _   _   _   _ =>
+      let eights: list (Tuplevector.t byte 8)
+                := map UInt64.uint64_to_le_bytes (a0 :: a1 :: a2 :: a3 :: nil)
+      in fold_right Tuplevector.app_to_list nil eights
+   end.
+
+Definition keccak_256 (data: list byte): list byte := squeeze_256 (absorb data 1).
+Definition sha3_256   (data: list byte): list byte := squeeze_256 (absorb data 6).
+
+Definition keccak_256_of_string (s: String.string)
+:= keccak_256 (bytes_of_string s).
+Definition sha3_256_of_string (s: String.string)
+:= sha3_256 (bytes_of_string s).
+
+Definition keccak_256_hex (data: list byte)
+: String.string
+:= hex_of_bytes (keccak_256 data) true.
+Definition sha3_256_hex (data: list byte)
+: String.string
+:= hex_of_bytes (sha3_256 data) true.
+
+Definition keccak_256_hex_of_string (s: String.string)
+: String.string
+:= hex_of_bytes (keccak_256_of_string s) true.
+Definition sha3_256_hex_of_string (s: String.string)
+: String.string
+:= hex_of_bytes (sha3_256_of_string s) true.
+
+(* This test is from Go's sha3_test.go. *)
+Example keccak_256_smoke_test:
+  keccak_256_hex_of_string "abc"
+   =
+  "4e03657aea45a94fc7d47ba826c8d667c0d1e6e33a64a036ec44f58fa12d6c45".
+Proof. trivial. Qed.
+
+(* A byte-long test from XKCP's ShortMsgKAT_SHA3-256.txt. *)
+Example sha3_256_test_CC:
+  sha3_256_hex (byte_of_N (HexString.to_N "0xCC") :: nil) 
+   = 
+  "677035391cd3701293d385f037ba32796252bb7ce180b00b582dd9b20aaad7f0".
+Proof. trivial. Qed.
