Hash/Nibble.v
@@ -1,0 +1,682 @@
+From Coq Require Import Ascii.
+From Coq Require Import NArith PArith ZArith.
+From Coq Require Import Int63.
+From Coq Require Import Lia.
+From Coq Require String Ascii.
+
+From Vyper Require Import UInt63 Arith2.
+
+Inductive nibble := Nibble (x3 x2 x1 x0: bool).
+Inductive hex_digit :=
+| x0 | x1 | x2 | x3
+| x4 | x5 | x6 | x7
+| x8 | x9 | xA | xB
+| xC | xD | xE | xF.
+
+Definition ascii_of_hex_digit (digit: hex_digit) (lower: bool)
+: ascii
+:= match digit with
+   | x0 => "0"
+   | x1 => "1"
+   | x2 => "2"
+   | x3 => "3"
+   | x4 => "4"
+   | x5 => "5"
+   | x6 => "6"
+   | x7 => "7"
+   | x8 => "8"
+   | x9 => "9"
+   | xA => if lower then "a" else "A"
+   | xB => if lower then "b" else "B"
+   | xC => if lower then "c" else "C"
+   | xD => if lower then "d" else "D"
+   | xE => if lower then "e" else "E"
+   | xF => if lower then "f" else "F"
+   end.
+
+Definition hex_digit_of_ascii (a: ascii)
+: option hex_digit
+:= match a with
+   | "0" => Some x0
+   | "1" => Some x1
+   | "2" => Some x2
+   | "3" => Some x3
+   | "4" => Some x4
+   | "5" => Some x5
+   | "6" => Some x6
+   | "7" => Some x7
+   | "8" => Some x8
+   | "9" => Some x9
+   | "a" | "A" => Some xA
+   | "b" | "B" => Some xB
+   | "c" | "C" => Some xC
+   | "d" | "D" => Some xD
+   | "e" | "E" => Some xE
+   | "f" | "F" => Some xF
+   | _ => None
+   end%char.
+
+Definition is_hex_digit (a: ascii)
+:= match hex_digit_of_ascii a with
+   | Some _ => true
+   | None => false
+   end.
+
+Lemma hex_digit_of_ascii_of_hex_digit (h: hex_digit) (lower: bool):
+  hex_digit_of_ascii (ascii_of_hex_digit h lower) = Some h.
+Proof.
+destruct lower; destruct h; trivial.
+Qed.
+
+Lemma is_hex_digit_true (a: ascii):
+  is_hex_digit a = true  ->  hex_digit_of_ascii a <> None.
+Proof.
+unfold is_hex_digit. now destruct hex_digit_of_ascii.
+Qed.
+
+Definition hex_digit_of_ascii' (a: ascii) (ok: is_hex_digit a = true)
+: hex_digit
+:= match hex_digit_of_ascii a as h return _ = h -> _ with
+   | Some x => fun _ => x
+   | None => fun E => False_rect _ (is_hex_digit_true a ok E)
+   end eq_refl.
+
+Lemma hex_digit_of_ascii_of_hex_digit' (h: hex_digit) (lower: bool)
+                                       (ok: is_hex_digit (ascii_of_hex_digit h lower) = true):
+  hex_digit_of_ascii' (ascii_of_hex_digit h lower) ok = h.
+Proof.
+destruct lower; destruct h; trivial.
+Qed.
+
+Definition nibble_of_hex_digit (digit: hex_digit)
+: nibble
+:= match digit with
+   | x0 => Nibble false false false false
+   | x1 => Nibble false false false true
+   | x2 => Nibble false false true  false
+   | x3 => Nibble false false true  true
+   | x4 => Nibble false true  false false
+   | x5 => Nibble false true  false true
+   | x6 => Nibble false true  true  false
+   | x7 => Nibble false true  true  true
+   | x8 => Nibble true  false false false
+   | x9 => Nibble true  false false true
+   | xA => Nibble true  false true  false
+   | xB => Nibble true  false true  true
+   | xC => Nibble true  true  false false
+   | xD => Nibble true  true  false true
+   | xE => Nibble true  true  true  false
+   | xF => Nibble true  true  true  true
+   end.
+
+Definition hex_digit_of_nibble (n: nibble)
+: hex_digit
+:= match n with
+   | Nibble false false false false => x0
+   | Nibble false false false true  => x1
+   | Nibble false false true  false => x2
+   | Nibble false false true  true  => x3
+   | Nibble false true  false false => x4
+   | Nibble false true  false true  => x5
+   | Nibble false true  true  false => x6
+   | Nibble false true  true  true  => x7
+   | Nibble true  false false false => x8
+   | Nibble true  false false true  => x9
+   | Nibble true  false true  false => xA
+   | Nibble true  false true  true  => xB
+   | Nibble true  true  false false => xC
+   | Nibble true  true  false true  => xD
+   | Nibble true  true  true  false => xE
+   | Nibble true  true  true  true  => xF
+   end.
+
+Lemma hex_digit_of_nibble_of_hex_digit (d: hex_digit):
+  hex_digit_of_nibble (nibble_of_hex_digit d) = d.
+Proof.
+destruct d; easy.
+Qed.
+
+Lemma nibble_of_hex_digit_of_nibble (n: nibble):
+  nibble_of_hex_digit (hex_digit_of_nibble n) = n.
+Proof.
+destruct n as (a3, a2, a1, a0).
+destruct a3; destruct a2; destruct a1; destruct a0; easy.
+Qed.
+
+Definition N_of_hex_digit (digit: hex_digit)
+: N 
+:= match digit with
+   | x0 =>  0
+   | x1 =>  1
+   | x2 =>  2
+   | x3 =>  3
+   | x4 =>  4
+   | x5 =>  5
+   | x6 =>  6
+   | x7 =>  7
+   | x8 =>  8
+   | x9 =>  9
+   | xA => 10
+   | xB => 11
+   | xC => 12
+   | xD => 13
+   | xE => 14
+   | xF => 15
+   end.
+
+Lemma N_of_hex_digit_ub (digit: hex_digit):
+  (N_of_hex_digit digit < 16)%N.
+Proof.
+  destruct digit; cbn; rewrite<- N.ltb_lt; trivial.
+Qed.
+
+Definition N_of_nibble (n: nibble)
+: N
+:= let f (a: bool) := if a then xI else xO in
+   match n with
+   | Nibble true a2 a1 a0 => Npos (f a0 (f a1 (f a2 xH)))
+   | Nibble false true a1 a0 => Npos (f a0 (f a1 xH))
+   | Nibble false false true a0 => Npos (f a0 xH)
+   | Nibble false false false true => Npos xH
+   | Nibble false false false false => N0
+   end.
+
+Lemma N_of_nibble_bound (n: nibble):
+  (N_of_nibble n < 16)%N.
+Proof.
+  destruct n as (a3, a2, a1, a0); destruct a3; destruct a2; destruct a1; destruct a0; easy.
+Qed.
+
+Lemma hex_digit_to_N_via_nibble (d: hex_digit):
+  N_of_nibble (nibble_of_hex_digit d) = N_of_hex_digit d.
+Proof.
+  destruct d; easy.
+Qed.
+
+Lemma nibble_to_N_via_hex_digit (n: nibble):
+  N_of_hex_digit (hex_digit_of_nibble n) = N_of_nibble n.
+Proof.
+  destruct n as (a3, a2, a1, a0); destruct a3; destruct a2; destruct a1; destruct a0; easy.
+Qed.
+
+Definition push_bit (n: N) (bit: bool)
+: N
+:= match n with
+   | N0 => if bit then 1 else 0
+   | Npos p => Npos ((if bit then xI else xO) p)
+   end.
+
+Lemma push_bit_arith (n: N) (bit: bool):
+  push_bit n bit = (2 * n + if bit then 1 else 0)%N.
+Proof.
+destruct bit; now destruct n.
+Qed.
+
+Definition last_bit (n: N)
+: bool
+:= match n with
+   | N0      | Npos (xO _) => false
+   | Npos xH | Npos (xI _) => true
+   end.
+
+Lemma last_bit_odd (n: N):
+  last_bit n = N.odd n.
+Proof.
+destruct n. { trivial. }
+destruct p; easy.
+Qed.
+
+Lemma push_bit_then_shr1 (n: N) (bit: bool):
+  N.div2 (push_bit n bit) = n.
+Proof.
+  destruct n; destruct bit; easy.
+Qed.
+
+Lemma last_of_push_bit (n: N) (bit: bool):
+  last_bit (push_bit n bit) = bit.
+Proof.
+  destruct n; destruct bit; easy.
+Qed.
+
+Lemma push_last_bit (n: N):
+  push_bit (N.div2 n) (last_bit n) = n.
+Proof.
+  destruct n. easy.
+  destruct p; easy.
+Qed.
+
+Definition push_nibble (n: N) (nib: nibble)
+: N
+:= match nib with
+   | Nibble a3 a2 a1 a0 => push_bit (push_bit (push_bit (push_bit n a3) a2) a1) a0
+   end.
+
+Lemma push_nibble_arith (n: N) (nib: nibble):
+  push_nibble n nib = (16 * n + N_of_nibble nib)%N.
+Proof.
+destruct nib as (a3, a2, a1, a0).
+unfold push_nibble.
+repeat rewrite push_bit_arith.
+repeat rewrite N.mul_add_distr_l.
+repeat rewrite<- N.add_assoc.
+f_equal.
+{ now repeat rewrite N.mul_assoc. }
+destruct a3; destruct a2; destruct a1; destruct a0; easy.
+Qed.
+
+Definition pop_nibble (n: N)
+: N * nibble
+:= let a0 := last_bit n in
+   let n1 := N.div2 n in
+   let a1 := last_bit n1 in
+   let n2 := N.div2 n1 in
+   let a2 := last_bit n2 in
+   let n3 := N.div2 n2 in
+   let a3 := last_bit n3 in
+   let n4 := N.div2 n3 in
+     (n4, Nibble a3 a2 a1 a0).
+
+Definition pop_hex_digit_pos (p: positive)
+: N * hex_digit
+:= (match p with
+    |  1 => (0%N, x1)
+    |  2 => (0%N, x2)
+    |  3 => (0%N, x3)
+    |  4 => (0%N, x4)
+    |  5 => (0%N, x5)
+    |  6 => (0%N, x6)
+    |  7 => (0%N, x7)
+    |  8 => (0%N, x8)
+    |  9 => (0%N, x9)
+    | 10 => (0%N, xA)
+    | 11 => (0%N, xB)
+    | 12 => (0%N, xC)
+    | 13 => (0%N, xD)
+    | 14 => (0%N, xE)
+    | 15 => (0%N, xF)
+    | q~0~0~0~0 => (N.pos q, x0)
+    | q~0~0~0~1 => (N.pos q, x1)
+    | q~0~0~1~0 => (N.pos q, x2)
+    | q~0~0~1~1 => (N.pos q, x3)
+    | q~0~1~0~0 => (N.pos q, x4)
+    | q~0~1~0~1 => (N.pos q, x5)
+    | q~0~1~1~0 => (N.pos q, x6)
+    | q~0~1~1~1 => (N.pos q, x7)
+    | q~1~0~0~0 => (N.pos q, x8)
+    | q~1~0~0~1 => (N.pos q, x9)
+    | q~1~0~1~0 => (N.pos q, xA)
+    | q~1~0~1~1 => (N.pos q, xB)
+    | q~1~1~0~0 => (N.pos q, xC)
+    | q~1~1~0~1 => (N.pos q, xD)
+    | q~1~1~1~0 => (N.pos q, xE)
+    | q~1~1~1~1 => (N.pos q, xF)
+    end)%positive.
+
+Definition pop_hex_digit (n: N)
+: N * hex_digit
+:= match n with
+   | 0%N => (0%N, x0)
+   | N.pos p => pop_hex_digit_pos p
+   end.
+
+Lemma pop_hex_digit_of_nibble (n: N):
+  pop_hex_digit n = let '(q, nib) := pop_nibble n in (q, hex_digit_of_nibble nib).
+Proof.
+destruct n. { easy. }
+destruct p; try destruct p; try destruct p; try destruct p; easy.
+Qed.
+
+Lemma push_nibble_then_pop (n: N) (nib: nibble):
+  pop_nibble (push_nibble n nib) = (n, nib).
+Proof.
+  destruct nib as (a3, a2, a1, a0). unfold pop_nibble. cbn.
+  repeat rewrite push_bit_then_shr1.
+  now repeat rewrite last_of_push_bit. 
+Qed.
+
+Lemma pop_nibble_then_push (n: N):
+  push_nibble (fst (pop_nibble n)) (snd (pop_nibble n)) = n.
+Proof.
+  destruct n. easy.
+  unfold pop_nibble. unfold fst. unfold snd.
+  unfold push_nibble.
+  now repeat rewrite push_last_bit.
+Qed.
+
+Definition nibble_of_N (n: N)
+: nibble
+:= snd (pop_nibble n).
+
+Lemma N_of_nibble_of_N (n: N) (B: (n < 16)%N):
+  N_of_nibble (nibble_of_N n) = n.
+Proof.
+assert(P := pop_nibble_then_push n).
+rewrite push_nibble_arith in P.
+unfold nibble_of_N.
+remember (N_of_nibble _) as k. clear Heqk.
+remember (fst _) as z. clear Heqz.
+lia.
+Qed.
+
+Definition pop_nibble_arith (a b: N) (B: (b < 16)%N):
+  pop_nibble (16 * a + b) = (a, nibble_of_N b).
+Proof.
+enough (E: push_nibble a (nibble_of_N b) = (16 * a + b)%N).
+{ rewrite<- E. apply push_nibble_then_pop. }
+rewrite push_nibble_arith.
+f_equal. apply N_of_nibble_of_N.
+assumption.
+Qed.
+
+Definition pop_nibble_arith_small (b: N) (B: (b < 16)%N):
+  pop_nibble b = (0%N, nibble_of_N b).
+Proof.
+rewrite<- (pop_nibble_arith _ _ B).
+f_equal.
+Qed.
+
+Definition nibble_of_uint63 (i: int)
+:= Nibble (0 < (i land 8))%int63
+          (0 < (i land 4))%int63
+          (0 < (i land 2))%int63
+          (0 < (i land 1))%int63.
+
+Definition uint63_of_nibble (n: nibble)
+:= match n with
+   | Nibble a8 a4 a2 a1 =>
+       ((if a8 then 8%int63 else 0%int63)
+         lor
+        (if a4 then 4%int63 else 0%int63)
+         lor
+        (if a2 then 2%int63 else 0%int63)
+         lor
+        (if a1 then 1%int63 else 0%int63))%int63
+   end.
+
+Lemma nibble_of_uint63_of_nibble (n: nibble):
+  nibble_of_uint63 (uint63_of_nibble n) = n.
+Proof.
+destruct n as (a3, a2, a1, a0).
+destruct a3; destruct a2; destruct a1; destruct a0; easy.
+Qed.
+
+(** A direct conversion from a native int to a hex digit via an if cascade. *)
+Definition hex_digit_of_uint63 (i: int)
+:= if (0 < (i land 8))%int63 then
+     if (0 < (i land 4))%int63 then
+       if (0 < (i land 2))%int63 then
+         if (0 < (i land 1))%int63 then xF else xE
+       else
+         if (0 < (i land 1))%int63 then xD else xC
+     else
+       if (0 < (i land 2))%int63 then
+         if (0 < (i land 1))%int63 then xB else xA
+       else
+         if (0 < (i land 1))%int63 then x9 else x8
+   else
+     if (0 < (i land 4))%int63 then
+       if (0 < (i land 2))%int63 then
+         if (0 < (i land 1))%int63 then x7 else x6
+       else
+         if (0 < (i land 1))%int63 then x5 else x4
+     else
+       if (0 < (i land 2))%int63 then
+         if (0 < (i land 1))%int63 then x3 else x2
+       else
+         if (0 < (i land 1))%int63 then x1 else x0.
+
+Lemma hex_digit_of_nibble_of_uint63 (i: int):
+  hex_digit_of_nibble (nibble_of_uint63 i) = hex_digit_of_uint63 i.
+Proof.
+unfold hex_digit_of_nibble. unfold nibble_of_uint63. unfold hex_digit_of_uint63.
+destruct (0 < i land 8)%int63;
+  destruct (0 < i land 4)%int63;
+  destruct (0 < i land 2)%int63;
+  destruct (0 < i land 1)%int63; easy.
+Qed.
+
+Lemma nibble_of_uint63_of_N (n: N):
+  nibble_of_uint63 (uint63_of_N n) = nibble_of_N n.
+Proof.
+unfold nibble_of_N. unfold pop_nibble. cbn.
+remember (uint63_of_N n) as i.
+unfold nibble_of_uint63.
+repeat rewrite last_bit_odd.
+repeat rewrite N.div2_spec.
+repeat rewrite N.shiftr_shiftr.
+repeat rewrite<- N.testbit_odd.
+rewrite<- N.bit0_odd.
+repeat rewrite uint63_testbit_N_low_digit; try lia.
+unfold get_digit. rewrite<- Heqi. cbn.
+f_equal; trivial.
+Qed.
+
+Lemma N_of_hex_digit_of_nibble (nib: nibble):
+  N_of_hex_digit (hex_digit_of_nibble nib) = N_of_nibble nib.
+Proof.
+destruct nib as (a, b, c, d).
+destruct a; destruct b; destruct c; destruct d; trivial.
+Qed.
+
+(***************************************************************************************)
+
+(* This is basically the standard Ascii thing except that bits are ordered MSB-to-LSB. *)
+Inductive byte := Byte (a7 a6 a5 a4 a3 a2 a1 a0: bool).
+
+Definition low_nibble (b: byte)
+: nibble
+:= match b with
+   | Byte _ _ _ _ a3 a2 a1 a0 => Nibble a3 a2 a1 a0
+   end.
+
+Definition high_nibble (b: byte)
+: nibble
+:= match b with
+   | Byte a7 a6 a5 a4 _ _ _ _ => Nibble a7 a6 a5 a4
+   end.
+
+Definition byte_of_nibbles (high low: nibble)
+: byte
+:= match high with
+   | Nibble a7 a6 a5 a4 =>
+      match low with
+      | Nibble a3 a2 a1 a0 =>
+         Byte a7 a6 a5 a4 a3 a2 a1 a0
+      end
+   end.
+
+Lemma low_nibble_ok (high low: nibble):
+  low_nibble (byte_of_nibbles high low) = low.
+Proof.
+  destruct low. destruct high. easy.
+Qed.
+
+Lemma high_nibble_ok (high low: nibble):
+  high_nibble (byte_of_nibbles high low) = high.
+Proof.
+  destruct low. destruct high. easy.
+Qed.
+
+Lemma byte_of_nibbles_ok (b: byte):
+  byte_of_nibbles (high_nibble b) (low_nibble b) = b.
+Proof.
+  now destruct b.
+Qed.
+
+Definition byte_of_hex_digits (high low: hex_digit)
+: byte
+:= byte_of_nibbles (nibble_of_hex_digit high) (nibble_of_hex_digit low).
+
+Definition hex_digits_of_byte (b: byte)
+: hex_digit * hex_digit
+:= (hex_digit_of_nibble (high_nibble b),
+    hex_digit_of_nibble (low_nibble b)).
+
+Definition N_of_byte (b: byte)
+: N
+:= let f (a: bool) := if a then xI else xO in
+   match b with
+   | Byte true a6 a5 a4 a3 a2 a1 a0 => Npos (f a0 (f a1 (f a2 (f a3 (f a4 (f a5 (f a6 xH)))))))
+   | Byte false true a5 a4 a3 a2 a1 a0 => Npos (f a0 (f a1 (f a2 (f a3 (f a4 (f a5 xH))))))
+   | Byte false false true a4 a3 a2 a1 a0 => Npos (f a0 (f a1 (f a2 (f a3 (f a4 xH)))))
+   | Byte false false false true a3 a2 a1 a0 => Npos (f a0 (f a1 (f a2 (f a3 xH))))
+   | Byte false false false false true a2 a1 a0 => Npos (f a0 (f a1 (f a2 xH)))
+   | Byte false false false false false true a1 a0 => Npos (f a0 (f a1 xH))
+   | Byte false false false false false false true a0 => Npos (f a0 xH)
+   | Byte false false false false false false false true => Npos xH
+   | Byte false false false false false false false false => N0
+   end.
+
+Definition pop_byte (n: N)
+: N * byte
+:= let (n1, x) := pop_nibble n in
+   let (n2, y) := pop_nibble n1 in
+     (n2, byte_of_nibbles y x).
+
+Definition byte_of_N (n: N)
+: byte
+:= snd (pop_byte n).
+
+Lemma byte_of_N_arith (high low: N)
+                       (H16: (high < 16)%N)
+                       (L16: (low < 16)%N):
+  byte_of_N (16 * high + low) = byte_of_nibbles (nibble_of_N high) (nibble_of_N low).
+Proof.
+unfold byte_of_N. unfold pop_byte.
+rewrite (pop_nibble_arith _ _ L16).
+remember (nibble_of_N low) as nib. clear Heqnib low L16.
+rewrite (pop_nibble_arith_small _ H16).
+trivial.
+Qed.
+
+Lemma byte_of_N_of_byte (b: byte):
+  byte_of_N (N_of_byte b) = b.
+Proof.
+destruct b as (a7, a6, a5, a4, a3, a2, a1, a0).
+destruct a7; destruct a6; destruct a5; destruct a4;
+destruct a3; destruct a2; destruct a1; destruct a0; trivial.
+Qed.
+
+Definition byte_of_int (i: int)
+:= Byte (0 < (i land 128))%int63
+        (0 < (i land 64))%int63
+        (0 < (i land 32))%int63
+        (0 < (i land 16))%int63
+        (0 < (i land 8))%int63
+        (0 < (i land 4))%int63
+        (0 < (i land 2))%int63
+        (0 < (i land 1))%int63.
+
+Definition int_of_byte (b: byte)
+:= match b with
+   | Byte b7 b6 b5 b4 b3 b2 b1 b0 =>
+     (let a7 := if b7 then 128 else 0 in
+      let a6 := if b6 then  64 lor a7 else a7 in
+      let a5 := if b5 then  32 lor a6 else a6 in
+      let a4 := if b4 then  16 lor a5 else a5 in
+      let a3 := if b3 then   8 lor a4 else a4 in
+      let a2 := if b2 then   4 lor a3 else a3 in
+      let a1 := if b1 then   2 lor a2 else a2 in
+                if b0 then   1 lor a1 else a1)%int63
+   end.
+
+Lemma byte_of_int_of_byte (b: byte):
+  byte_of_int (int_of_byte b) = b.
+Proof.
+destruct b as (a7, a6, a5, a4, a3, a2, a1, a0).
+destruct a7; destruct a6; destruct a5; destruct a4;
+destruct a3; destruct a2; destruct a1; destruct a0; trivial.
+Qed.
+
+Fixpoint hex_of_bytes (b: list byte) (lower: bool)
+: String.string
+:= match b with
+   | nil => String.EmptyString
+   | (h :: t)%list =>
+        let (hi, lo) := hex_digits_of_byte h in
+          String.String (ascii_of_hex_digit hi lower)
+                        (String.String (ascii_of_hex_digit lo lower)
+                                       (hex_of_bytes t lower))
+   end.
+
+Definition byte_of_ascii (a: ascii)
+:= let (b0, b1, b2, b3, b4, b5, b6, b7) := a in Byte b7 b6 b5 b4 b3 b2 b1 b0.
+
+Fixpoint bytes_of_string (s: String.string)
+: list byte
+:= match s with
+   | String.EmptyString => nil
+   | String.String h t => byte_of_ascii h :: bytes_of_string t
+   end.
+
+(* TODO: to Str *)
+Fixpoint string_forallb (f: ascii -> bool) (s: String.string)
+: bool
+:= match s with
+   | String.EmptyString => true
+   | String.String h t => f h && string_forallb f t
+   end.
+
+Lemma string_forallb_iff (f: ascii -> bool) (s: String.string):
+  string_forallb f s = List.forallb f (String.list_ascii_of_string s).
+Proof.
+induction s; cbn. { trivial. }
+f_equal. exact IHs.
+Qed.
+
+Definition is_hex_string (s: String.string)
+: bool
+:= Nat.even (String.length s) 
+    &&
+   string_forallb is_hex_digit s.
+
+Fixpoint bytes_of_hex (s: String.string)
+                       (ok: is_hex_string s = true)
+: list byte.
+Proof.
+refine(match s as s' return s = s' -> _ with
+       | String.EmptyString => fun _ => nil
+       | String.String h String.EmptyString => fun E => _
+       | String.String hi (String.String lo rest) => fun E =>
+           (byte_of_hex_digits (hex_digit_of_ascii' hi _) (hex_digit_of_ascii' lo _)
+            ::
+            bytes_of_hex rest _)%list
+       end eq_refl); 
+  unfold is_hex_string in ok; unfold string_forallb in ok; subst; cbn in *;
+  repeat (rewrite Bool.andb_true_iff in *); try easy.
+fold string_forallb in ok. unfold is_hex_string.
+rewrite Bool.andb_true_iff.
+tauto.
+Defined.
+
+Lemma ascii_of_hex_digit_is_hex_digit (h: hex_digit) (lower: bool):
+  is_hex_digit (ascii_of_hex_digit h lower) = true.
+Proof.
+unfold is_hex_digit. now rewrite hex_digit_of_ascii_of_hex_digit.
+Qed.
+
+Lemma hex_of_bytes_is_hex_string (b: list byte) (lower: bool)
+: is_hex_string (hex_of_bytes b lower) = true.
+Proof.
+unfold is_hex_string. repeat (rewrite Bool.andb_true_iff).
+split; induction b; try easy.
+cbn. repeat rewrite ascii_of_hex_digit_is_hex_digit.
+rewrite IHb. trivial.
+Qed.
+
+Lemma bytes_of_hex_of_bytes (b: list byte) (lower: bool):
+  let hex := hex_of_bytes b lower in
+  forall ok: is_hex_string hex = true,
+    bytes_of_hex hex ok = b.
+Proof.
+induction b. { easy. }
+cbn zeta in *. intro ok.
+cbn. f_equal.
+{
+  unfold byte_of_hex_digits.
+  repeat rewrite hex_digit_of_ascii_of_hex_digit'.
+  repeat rewrite nibble_of_hex_digit_of_nibble.
+  apply byte_of_nibbles_ok.
+}
+apply IHb.
+Qed.
