Hash/Tuplevector.v
@@ -1,0 +1,247 @@
+From Coq Require Import Arith.
+From Coq Require List.
+
+(** A tuplevector is a tuple containing items of the same type. *)
+Fixpoint t (T: Type) (n: nat)
+: Type
+:= match n with
+   | O => unit
+   | 1%nat => T
+   | S k => (t T k * T)%type
+   end.
+
+(** The tuplevector type simply expands to a power of its base type: *)
+Local Example type_example: t nat 3 = (nat * nat * nat)%type.
+Proof. trivial. Qed.
+
+(** Coq already has a notation for a tuplevector. The type needs to be supplied though. *)
+Local Example example_tuple_5: t nat 5 := (10, 20, 30, 40, 50).
+
+(** As an exception, a tuple with one item is just the item itself.
+    In Lisp terms, a tuple is an improper list (also backwards, that is,
+    the head is in the rightmost position).
+ *)
+Local Example example_tuple_1: t nat 1 := 10.
+
+(** Let can destructure a tuplevector with an apostrophe: *)
+Local Example destructuring_example:
+  (let tuple := (10, 20, 30, 40, 50): t nat 5 in
+   let '(a, b, c, d, e) := tuple in 
+   a) 
+    = 
+  10.
+Proof. trivial. Qed.
+
+(** [snoc] is a term from Haskell, it means cons backwards. *)
+Definition snoc {T n} (tv: t T n) (last: T)
+: t T (S n)
+:= match n, tv with
+   | 0, _ => last
+   | S _, x => (x, last)
+   end.
+
+Local Example snoc_example:
+  snoc ((10, 20, 30): t nat 3) 40 = (10, 20, 30, 40).
+Proof. trivial. Qed.
+
+Definition last {T n} (tv: t T (S n))
+: T
+:= match n, tv with
+   | 0, x => x
+   | S _, (_, x) => x
+   end.
+
+Lemma last_of_snoc {T n} (tv: t T n) (x: T):
+  last (snoc tv x) = x.
+Proof.
+destruct n; easy.
+Qed.
+
+Definition but_last {T n} (tv: t T (S n))
+: t T n
+:= match n, tv with
+   | 0, x => tt
+   | S k, (rest, x) => rest
+   end.
+
+Lemma but_last_of_snoc {T n} (tv: t T n) (x: T):
+  but_last (snoc tv x) = tv.
+Proof.
+destruct n. { now destruct tv. }
+destruct n; easy.
+Qed.
+
+Lemma snoc_ok {T n} (tv: t T (S n)):
+  snoc (but_last tv) (last tv) = tv.
+Proof.
+destruct n. { easy. }
+now destruct tv.
+Qed.
+
+Fixpoint app_to_list {T n} (tv: t T n) (l: list T)
+: list T
+:= match n as n' return (t T n' -> list T) with
+   | 0 => fun _ => l
+   | S k => fun tv' => app_to_list (but_last tv') (last tv' :: l)%list
+   end tv.
+
+Local Example app_to_list_example:
+  app_to_list ((5, 15): t _ 2) (10 :: 20 :: 30 :: nil)%list = (5 :: 15 :: 10 :: 20 :: 30 :: nil)%list.
+Proof. trivial. Qed.
+
+Lemma app_to_list_length {T n} (tv: t T n) (l: list T):
+  length (app_to_list tv l) = n + length l.
+Proof.
+revert l.
+induction n. { easy. }
+cbn. intros. rewrite IHn. cbn.
+symmetry. apply plus_n_Sm.
+Qed.
+
+Fixpoint prepend {T: Type} {n: nat} (new: T) (tv: t T n)
+: t T (S n)
+:= match n, tv with
+   | 0, _ => new
+   | S _, x => (prepend new (but_last x), last x)
+   end.
+
+Local Example prepend_example:
+  prepend 5 ((2, 3, 4): t nat 3) = (5, 2, 3, 4).
+Proof. trivial. Qed.
+
+Fixpoint rev {T: Type} {n: nat} (tv: t T n)
+: t T n
+:= match n, tv with
+   | 0, _ => tt
+   | S _, x => prepend (last x) (rev (but_last x))
+   end.
+
+Local Example rev_example:
+   rev ((1, 2, 3, 4): t nat 4) = (4, 3, 2, 1).
+Proof. trivial. Qed.
+
+(************************************************)
+
+Local Lemma take_from_list_helper {T k} {head: T} {tail: list T}
+                                   (H: S k <= length (head :: tail)%list):
+  k <= length tail.
+Proof.
+apply le_S_n. apply H.
+Qed. 
+
+Fixpoint take_from_list_rev {T n} (l: list T) (ok: n <= length l)
+: t T n * list T
+:= match n as n' return n' <= length l -> t T n' * list T with
+   | O => fun _ => (tt, l)
+   | S k =>
+      match l as l' return S k <= length l' -> t T (S k) * list T with
+      | nil => fun X => False_rect _ (Nat.nle_succ_0 k X)
+      | (head :: tail)%list => fun X =>
+           let (prefix, rest) := take_from_list_rev tail (take_from_list_helper X) in
+           (snoc prefix head, rest)
+      end
+   end ok.
+
+Fixpoint to_list_backwards {T n} (tv: t T n)
+: list T
+:= match n, tv with
+   | 0, _ => nil
+   | S _, x => last x :: to_list_backwards (but_last x)
+   end.
+
+Local Example to_list_backwards_example:
+   to_list_backwards ((1, 2, 3, 4): t nat 4) = (4 :: 3 :: 2 :: 1 :: nil)%list.
+Proof. trivial. Qed.
+
+Lemma take_from_list_rev_firstn {T n} (l: list T) (ok: n <= length l):
+  to_list_backwards (fst (take_from_list_rev l ok)) = List.firstn n l.
+Proof.
+revert l ok. induction n, l; try easy. intros.
+cbn.
+assert (M := IHn l (take_from_list_helper ok)).
+remember (take_from_list_rev l (take_from_list_helper ok)) as pq. destruct pq as (p, q).
+cbn in *.
+rewrite last_of_snoc. rewrite but_last_of_snoc. f_equal.
+exact M.
+Qed.
+
+Lemma take_from_list_rev_skipn {T n} (l: list T) (ok: n <= length l):
+  snd (take_from_list_rev l ok) = List.skipn n l.
+Proof.
+revert l ok. induction n, l; try easy. intros.
+cbn.
+assert (M := IHn l (take_from_list_helper ok)).
+remember (take_from_list_rev l (take_from_list_helper ok)) as pq. destruct pq as (p, q).
+cbn in *. exact M.
+Qed.
+
+(** This function fixes the flip of take_from_list_rev by applying rev.
+    The name reflects the opinion that this function should be avoided 
+    because rev is quadratic.
+ *)
+Definition take_from_list_slow {T n} (l: list T) (ok: n <= length l)
+: t T n * list T
+:= let (prefix, rest) := take_from_list_rev l ok
+   in (rev prefix, rest).
+
+(**********************************************************************************)
+
+Local Lemma gather_helper_nil {T} {x: T} {l: list T} {block_len}:
+  ~ (length (x :: l) = 0 * block_len).
+Proof. discriminate. Qed.
+
+Local Lemma gather_helper_block_len {T} (k block_len: nat) (l: list T)
+                                     (E : length l = S k * block_len):
+  block_len <= length l.
+Proof. 
+rewrite E.
+rewrite<- Nat.mul_1_l at 1.
+apply Nat.mul_le_mono_r.  
+apply le_n_S.
+apply Nat.le_0_l.
+Qed.
+
+Definition take_from_list_rev_dep_skipn {T n} (l: list T) (ok: n <= length l)
+: { x: t T n * list T | snd x = List.skipn n l }
+:= exist _ (take_from_list_rev l ok) (take_from_list_rev_skipn l ok).
+
+Local Lemma gather_helper_skipn {T k block_len l}
+            (ok: length l = S k * block_len)
+            (p: {x : t T block_len * list T | snd x = List.skipn block_len l}):
+  length (snd (proj1_sig p)) = k * block_len.
+Proof.
+assert (P := proj2_sig p). cbn in P. rewrite P.
+rewrite List.skipn_length.
+rewrite ok.
+cbn.
+rewrite Nat.add_comm.
+rewrite Nat.add_sub.
+trivial.
+Qed.
+
+Fixpoint gather {T} (l: list T) (n block_len: nat) (ok: length l = n * block_len)
+{struct n}
+: list (t T block_len)
+:= match n as n' return length l = n' * block_len -> list (t T block_len) with
+   | O => match l as l' return length l' = 0 * block_len -> _ with
+          | nil => fun _ => nil
+          | cons _ _ => fun ok' => False_rect _ (gather_helper_nil ok')
+          end
+   | S k => fun ok' =>
+              let p := take_from_list_rev_dep_skipn l (gather_helper_block_len k block_len l ok') in
+              (fst (proj1_sig p) :: gather (snd (proj1_sig p)) k block_len
+                                           (gather_helper_skipn ok' p))%list
+   end ok.
+
+Example gather_example:
+  gather (1 :: 2 :: 3 :: 4 :: 5 :: 6 :: 7 :: 8 :: 9 :: 10 :: nil)%list 5 2 eq_refl
+   =
+  ((2, 1) :: (4, 3) :: (6, 5) :: (8, 7) :: (10, 9) :: nil)%list.
+Proof. trivial. Qed.
+
+Lemma gather_length {T} (l: list T) (n block_len: nat) (ok: length l = n * block_len):
+  List.length (gather l n block_len ok) = n.
+Proof.
+revert l ok. induction n; intros; destruct l; cbn;
+  trivial; try easy; f_equal; apply IHn.
+Qed.
