Hash/UInt63.v
@@ -1,0 +1,264 @@
+(** 
+  This file continues theories/Numbers/Cyclic/Int63/Int63.v from the standard library of Coq.
+ *)
+
+From Coq Require Import Int63 NArith ZArith Lia.
+
+From Vyper Require Import Logic2 Arith2.
+
+Definition uint63 := int.
+Definition Z_of_uint63 := to_Z.
+Definition uint63_of_Z := of_Z.
+
+Ltac rewrite_Z_of_uint63 
+:= repeat (rewrite lsl_spec
+        || rewrite lsr_spec
+        || rewrite land_spec'
+        || rewrite lor_spec'
+        || rewrite lxor_spec'
+        || rewrite add_spec
+        || rewrite sub_spec
+        || rewrite mul_spec
+        || rewrite div_spec
+        || rewrite mod_spec
+        || rewrite ltb_spec
+        || rewrite leb_spec).
+
+Definition N_of_uint63 (i: uint63): N
+:= Z.to_N (to_Z i).
+Definition uint63_of_N (n: N): uint63
+:= of_Z (Z.of_N n).
+
+Definition nat_of_uint63 (i: uint63): nat
+:= N.to_nat (N_of_uint63 i).
+
+Definition uint63_of_nat (n: nat): uint63
+:= uint63_of_N (N.of_nat n).
+
+
+Lemma Z_of_uint63_nonneg (i: uint63):
+  (0 <= to_Z i)%Z.
+Proof.
+assert(B := to_Z_bounded i).
+tauto.
+Qed.
+
+Lemma uint63_ltb_Z (x y: uint63):
+  (x < y)%int63 = (to_Z x <? to_Z y)%Z.
+Proof.
+apply (relation_quad (fun x y => iff_refl _) Z.ltb_lt).
+apply ltb_spec.
+Qed.
+
+Lemma uint63_leb_Z (x y: uint63):
+  (x <= y)%int63 = (to_Z x <=? to_Z y)%Z.
+Proof.
+apply (relation_quad (fun x y => iff_refl _) Z.leb_le).
+apply leb_spec.
+Qed.
+
+Lemma uint63_ltb_N (x y: uint63):
+  (x < y)%int63 = (N_of_uint63 x <? N_of_uint63 y)%N.
+Proof.
+rewrite uint63_ltb_Z.
+unfold N_of_uint63.
+assert (Bx := to_Z_bounded x).
+assert (By := to_Z_bounded y).
+destruct Bx as (Bx, _).
+destruct By as (By, _).
+assert (L := Z2N.inj_lt (to_Z x) (to_Z y) Bx By).
+clear Bx By.
+apply (relation_quad Z.ltb_lt N.ltb_lt).
+apply L.
+Qed.
+
+Lemma uint63_leb_N (x y: uint63):
+  (x <= y)%int63 = (N_of_uint63 x <=? N_of_uint63 y)%N.
+Proof.
+rewrite uint63_leb_Z.
+unfold N_of_uint63.
+assert (Bx := to_Z_bounded x).
+assert (By := to_Z_bounded y).
+destruct Bx as (Bx, _).
+destruct By as (By, _).
+assert (L := Z2N.inj_le (to_Z x) (to_Z y) Bx By).
+clear Bx By.
+apply (relation_quad Z.leb_le N.leb_le).
+apply L.
+Qed.
+
+Lemma uint63_get_high_digit (i k: uint63)
+                            (B: (63 <= k)%int63 = true):
+  get_digit i k = false.
+Proof.
+unfold get_digit.
+enough (U: (1 << k = 0)%int63).
+{ 
+  rewrite U.
+  rewrite uint63_ltb_Z.
+  rewrite land_spec'.
+  rewrite to_Z_0.
+  rewrite Z.land_0_r.
+  trivial.
+}
+match goal with
+|- ?lhs = ?rhs => rewrite<- (of_to_Z lhs); rewrite<- (of_to_Z rhs)
+end.
+f_equal.
+rewrite lsl_spec.
+rewrite to_Z_1. rewrite to_Z_0.
+rewrite Z.mul_1_l.
+rewrite uint63_leb_Z in B.
+replace (to_Z 63%int63) with 63%Z in B. 2:{ trivial. }
+remember (to_Z k) as n. clear i k Heqn.
+remember (n - 63)%Z as m.
+assert (Q: n = (m + 63)%Z). { subst. lia. }
+subst n.
+rewrite Z.pow_add_r; rewrite Z.leb_le in B; [ | lia | lia ].
+apply Z_mod_mult.
+Qed.
+
+Lemma uint63_testbit_Z (i k: uint63):
+  get_digit i k = Z.testbit (to_Z i) (to_Z k).
+Proof.
+remember (k < 63)%int63 as Low. symmetry in HeqLow.
+destruct Low.
+{ 
+  unfold get_digit.
+  rewrite uint63_ltb_Z.
+  rewrite land_spec'.
+  rewrite lsl_spec.
+  remember (to_Z i) as n.
+  remember (to_Z k) as m.
+  replace (to_Z 0%int63) with 0%Z. 2:{ trivial. }
+  replace (to_Z 1%int63) with 1%Z. 2:{ trivial. }
+  rewrite Z.mul_1_l.
+  rewrite Z.mod_small.
+  2:{
+    split. { apply Z.pow_nonneg. rewrite<- Z.leb_le. trivial. }
+    unfold wB.
+    apply Z.pow_lt_mono_r.
+    { rewrite<- Z.ltb_lt. trivial. }
+    { rewrite<- Z.leb_le. trivial. }
+    subst.
+    rewrite ltb_spec in HeqLow.
+    assumption.
+}
+symmetry.
+apply Z_testbit_alt.
+assert (BN := to_Z_bounded i).
+subst. tauto.
+assert (BM := to_Z_bounded k).
+subst. tauto.
+}
+assert(Bk: (63 <= to_Z k)%Z).
+{
+  rewrite uint63_ltb_Z in HeqLow.
+  replace (to_Z 63%int63) with 63%Z in HeqLow. 2:{ trivial. }
+  rewrite Z.ltb_ge in HeqLow.
+  assumption.
+}
+rewrite uint63_get_high_digit.
+{
+  symmetry.
+  assert(Bi := to_Z_bounded i).
+  apply Z_testbit_high.
+  { assert(BK := to_Z_bounded k). tauto. }
+  split. { tauto. }
+  apply (Z.lt_le_trans _ wB _). { tauto. }
+  apply Z.pow_le_mono_r. { rewrite<- Z.ltb_lt. trivial. }
+  apply Bk.
+}
+rewrite leb_spec.
+apply Bk.
+Qed.
+
+Lemma uint63_testbit_N_low_digit (n k: N)
+                                  (B: (k < 63)%N):
+  N.testbit n k = get_digit (uint63_of_N n) (uint63_of_N k).
+Proof.
+rewrite<- N2Z.inj_testbit.
+rewrite uint63_testbit_Z.
+unfold uint63_of_N.
+repeat rewrite of_Z_spec.
+rewrite (Z.mod_small (Z.of_N k)). 2:{ unfold wB. cbn. lia. }
+symmetry.
+apply Z.mod_pow2_bits_low.
+unfold size.
+lia.
+Qed.
+
+Lemma uint63_bit_get_digit (i k: uint63):
+  bit i k = get_digit i k.
+Proof.
+rewrite bitE. rewrite uint63_testbit_Z. trivial.
+Qed.
+
+(**************************************************************************)
+
+Lemma uint63_land_N (x y: uint63):
+  N_of_uint63 (x land y)%int63 = N.land (N_of_uint63 x) (N_of_uint63 y).
+Proof.
+unfold N_of_uint63.
+rewrite land_spec'.
+apply Z_to_N_land; apply Z_of_uint63_nonneg.
+Qed.
+
+Lemma uint63_lor_N (x y: uint63):
+  N_of_uint63 (x lor y)%int63 = N.lor (N_of_uint63 x) (N_of_uint63 y).
+Proof.
+unfold N_of_uint63.
+rewrite lor_spec'.
+apply Z_to_N_lor; apply Z_of_uint63_nonneg.
+Qed.
+
+Lemma uint63_lxor_N (x y: uint63):
+  N_of_uint63 (x lxor y)%int63 = N.lxor (N_of_uint63 x) (N_of_uint63 y).
+Proof.
+unfold N_of_uint63.
+rewrite lxor_spec'.
+apply Z_to_N_lxor; apply Z_of_uint63_nonneg.
+Qed.
+
+(**************************************************************************)
+
+Lemma uint63_add_sub_assoc (n m p: int):
+  (n + (m - p))%int63 = (n + m - p)%int63.
+Proof.
+apply to_Z_inj.
+repeat (rewrite add_spec || rewrite sub_spec).
+rewrite Z.add_mod_idemp_r by discriminate.
+repeat rewrite<- Z.add_opp_r.
+rewrite Z.add_mod_idemp_l by discriminate.
+now rewrite Z.add_assoc.
+Qed.
+
+Lemma uint63_add_opp_r (n m: int):
+  (n + - m)%int63 = (n - m)%int63.
+Proof.
+apply to_Z_inj.
+repeat (rewrite add_spec || rewrite sub_spec || rewrite opp_spec).
+rewrite Z.add_mod_idemp_r by discriminate.
+now repeat rewrite Z.add_opp_r.
+Qed.
+
+Lemma uint63_to_Z_ne_0 (n: int) (NZ: n <> 0%int63):
+  to_Z n <> 0%Z.
+Proof.
+intro H.
+rewrite<- (of_to_Z n) in NZ.
+rewrite H in NZ.
+cbn in NZ.
+contradiction.
+Qed.
+
+Lemma uint63_dec_to_Z (n: int) (NZ: n <> 0%int63):
+  to_Z (n - 1) = (to_Z n - 1)%Z.
+Proof.
+rewrite sub_spec.
+replace (to_Z 1%int63) with 1%Z by trivial.
+apply Z.mod_small.
+assert (A := to_Z_bounded n).
+assert (P := uint63_to_Z_ne_0 n NZ).
+lia.
+Qed.
