Hash/UInt64.v
@@ -1,0 +1,726 @@
+From Coq Require Import ZArith Lia.
+From Coq Require Import Int63.
+From Coq Require Bool.
+From Coq Require Import CyclicAxioms.
+
+From Vyper Require Import Arith2 UInt63 Nibble.
+
+Definition uint64 := (bool * int)%type.
+Definition t := uint64.
+
+Local Open Scope Z_scope.
+
+Definition Z_of_uint64 (a: uint64)
+:= match a with
+   | (false, n) => Int63.to_Z n
+   | (true , n) => Int63.to_Z n + Int63.wB
+   end.
+
+Definition Z_of_uint64_lor (a: uint64)
+:= match a with
+   | (false, n) => Int63.to_Z n
+   | (true , n) => Z.lor (Int63.to_Z n) Int63.wB
+   end.
+
+Lemma Z_of_uint64_lor_ok (a: uint64):
+  Z_of_uint64_lor a = Z_of_uint64 a.
+Proof.
+unfold Z_of_uint64_lor.
+destruct a as (b, n).
+rewrite<- Arith2.Z_add_nocarry_lor. { trivial. }
+apply Arith2.Z_land_pow2_small. { apply to_Z_bounded. }
+apply Nat2Z.is_nonneg.
+Qed.
+
+Definition Z_of_uint64_lxor (a: uint64)
+:= match a with
+   | (false, n) => Int63.to_Z n
+   | (true , n) => Z.lxor (Int63.to_Z n) Int63.wB
+   end.
+
+Lemma Z_of_uint64_lxor_ok (a: uint64):
+  Z_of_uint64_lxor a = Z_of_uint64 a.
+Proof.
+unfold Z_of_uint64_lxor.
+destruct a as (b, n).
+rewrite<- Z.add_nocarry_lxor. { trivial. }
+apply Arith2.Z_land_pow2_small. { apply to_Z_bounded. }
+apply Nat2Z.is_nonneg.
+Qed.
+
+Lemma Z_of_uint64_lower (a: uint64):
+  0 <= Z_of_uint64 a.
+Proof.
+destruct a as (hi, lo).
+assert(B := Int63.to_Z_bounded lo).
+destruct B as (L, H).
+destruct hi; unfold Z_of_uint64; lia.
+Qed.
+
+Lemma Z_of_uint64_upper (a: uint64):
+  Z_of_uint64 a < 2^64.
+Proof.
+destruct a as (hi, lo).
+assert(B := Int63.to_Z_bounded lo).
+destruct B as (_, H).
+assert (E: Int63.wB = 2^63). { unfold Int63.wB. f_equal. }
+destruct hi; unfold Z_of_uint64; lia.
+Qed.
+
+Definition Z_of_uint64' (a: uint64)
+:= let (b, n) := a in
+   Int63.to_Z n + (if b then 1 else 0) * Int63.wB.
+
+Lemma Z_of_uint64_alt (a: uint64):
+  Z_of_uint64' a = Z_of_uint64 a.
+Proof.
+unfold Z_of_uint64'. unfold Z_of_uint64.
+destruct a as (b, n). destruct b; lia.
+Qed.
+
+Definition Z_of_uint64_lor' (a: uint64)
+:= let (b, n) := a in
+   Z.lor (Int63.to_Z n) ((if b then 1 else 0) * Int63.wB).
+
+Lemma Z_of_uint64_lor'_ok (a: uint64):
+  Z_of_uint64_lor' a = Z_of_uint64' a.
+Proof.
+unfold Z_of_uint64_lor'.
+destruct a as (b, n).
+rewrite<- Arith2.Z_add_nocarry_lor. { trivial. }
+destruct b.
+{
+  rewrite Z.mul_1_l. apply Arith2.Z_land_pow2_small. 
+  { apply to_Z_bounded. } apply Nat2Z.is_nonneg.
+}
+rewrite Z.mul_0_l. rewrite Z.land_0_r. trivial.
+Qed.
+
+Definition uint64_of_Z (z: Z)
+                        (lower: 0 <= z)
+                        (upper: z < 2^64)
+: uint64
+:= (2^63 <=? z, Int63.of_Z z).
+
+Lemma uint64_of_Z_of_uint64 (a: uint64):
+  uint64_of_Z (Z_of_uint64 a) (Z_of_uint64_lower a) (Z_of_uint64_upper a) = a.
+Proof.
+assert (E: Int63.wB = 2^63). { unfold Int63.wB. f_equal. }
+destruct a as (hi, lo).
+assert(B := Int63.to_Z_bounded lo).
+destruct hi; unfold Z_of_uint64; unfold uint64_of_Z.
+{
+  rewrite E. f_equal.
+  { rewrite Z.leb_le. lia. }
+  rewrite<- E. clear E.
+  apply Int63.to_Z_inj. rewrite Int63.of_Z_spec.
+  rewrite Z.add_comm.
+  rewrite<- Zplus_mod_idemp_l.
+  rewrite Z_mod_same_full.
+  rewrite Z.add_0_l.
+  remember (Int63.to_Z lo) as n. clear Heqn.
+  exact (Z.mod_small _ _ B).
+}
+rewrite<- E.
+f_equal. { rewrite Z.leb_gt. tauto. }
+apply Int63.of_to_Z.
+Qed.
+
+Lemma Z_of_uint64_of_Z (z: Z)
+                        (lower: 0 <= z)
+                        (upper: z < 2^64):
+  Z_of_uint64 (uint64_of_Z z lower upper) = z.
+Proof.
+assert (E: Int63.wB = 2^63). { unfold Int63.wB. f_equal. }
+unfold Z_of_uint64. unfold uint64_of_Z.
+remember (2 ^ 63 <=? z) as is_high.
+rewrite Int63.of_Z_spec.
+symmetry in Heqis_high.
+destruct is_high.
+{
+  rewrite Z.leb_le in Heqis_high.
+  rewrite E. clear E.
+  remember (z - 2^63) as y.
+  assert (YL: 0 <= y) by lia.
+  assert (YU: y < 2^63) by lia.
+  assert (R: z mod 2^63 = y mod 2^63).
+  {
+    subst.
+    rewrite<- Zminus_mod_idemp_r.
+    rewrite Z_mod_same_full.
+    rewrite Z.sub_0_r.
+    trivial.
+  }
+  rewrite R.
+  rewrite (Z.mod_small _ _ (conj YL YU)).
+  lia.
+}
+rewrite Z.leb_gt in Heqis_high.
+apply Z.mod_small. tauto.
+Qed.
+
+Definition uint64_of_Z_mod (z: Z)
+: uint64
+:= (Z.testbit z 63, Int63.of_Z z).
+
+Lemma uint64_mod_pos_bound (a: Z):
+  0 <= a mod 2^64 < 2^64.
+Proof.
+apply Z.mod_pos_bound.
+rewrite<- Z.ltb_lt.
+trivial.
+Qed.
+ 
+Lemma uint64_of_Z_mod_ok (z: Z):
+  uint64_of_Z_mod z = uint64_of_Z (z mod 2^64)
+                                  (proj1 (uint64_mod_pos_bound z))
+                                  (proj2 (uint64_mod_pos_bound z)).
+Proof.
+unfold uint64_of_Z. unfold uint64_of_Z_mod.
+f_equal.
+{
+  rewrite<- (Z.mod_pow2_bits_low z 64 63) by now rewrite<- Z.ltb_lt.
+  assert (B := uint64_mod_pos_bound z).
+  remember (z mod 2 ^ 64) as x. clear Heqx.
+  rewrite (Z.testbit_odd x 63).
+  rewrite Z.shiftr_div_pow2 by now rewrite<- Z.leb_le.
+  remember (2 ^ 63 <=? x) as f. symmetry in Heqf.
+  destruct f.
+  {
+    rewrite Z.leb_le in Heqf.
+    assert(L: 1 <= x / 2 ^ 63).
+    {
+      rewrite<- (Z.div_same (2^63)) by discriminate.
+      apply Z.div_le_mono. { rewrite<- Z.ltb_lt. trivial. }
+      assumption.
+    }
+    assert (U: x / 2^63 <= (2 ^ 64 - 1) / 2 ^ 63).
+    {
+      apply Z.div_le_mono. { rewrite<- Z.ltb_lt. trivial. }
+      lia.
+    }
+    replace ((2 ^ 64 - 1) / 2 ^ 63) with 1 in U by trivial.
+    assert (E: x / 2 ^ 63 = 1) by lia.
+    now rewrite E.
+  }
+  rewrite (Logic2.b_false (Z.leb_le _ _)) in Heqf.
+  apply Z.nle_gt in Heqf.
+  replace (x / 2 ^ 63) with 0. 2:{ symmetry. apply Z.div_small. tauto. }
+  trivial.
+}
+apply to_Z_inj.
+repeat rewrite of_Z_spec. 
+apply Znumtheory.Zmod_div_mod; try rewrite<- Z.ltb_lt; trivial.
+replace (2^64) with (2 * wB) by trivial.
+apply Z.divide_factor_r.
+Qed.
+
+Lemma Z_of_uint64_of_Z_mod (z: Z):
+  Z_of_uint64 (uint64_of_Z_mod z) = z mod 2^64.
+Proof.
+rewrite uint64_of_Z_mod_ok.
+rewrite Z_of_uint64_of_Z.
+trivial.
+Qed.
+
+Definition uint64_0: uint64 := (false, 0%int63).
+Lemma uint64_0_ok:
+  Z_of_uint64 uint64_0 = 0.
+Proof. trivial. Qed.
+Definition uint64_1: uint64 := (false, 1%int63).
+Lemma uint64_1_ok:
+  Z_of_uint64 uint64_1 = 1.
+Proof. trivial. Qed.
+Definition uint64_max_value: uint64 := (true, max_int).
+Lemma uint64_max_value_ok:
+  Z_of_uint64 uint64_max_value = 2^64 - 1.
+Proof. trivial. Qed.
+
+(*******************************************************************************)
+
+Definition add (a b: uint64)
+: uint64
+:= let (ha, la) := a in
+   let (hb, lb) := b in
+   let x := xorb ha hb in
+   match Int63.addc la lb with
+   | DoubleType.C0 c => (x, c)
+   | DoubleType.C1 c => (negb x, c)
+   end.
+
+Ltac wB_up
+:= repeat (rewrite (Z.add_comm _ Int63.wB)
+        || rewrite (Z.add_comm _ (_ * Int63.wB)));
+   repeat rewrite Z.add_assoc;
+   repeat rewrite<- Z.mul_add_distr_r.
+
+Lemma mod_wB (x: Z):
+  (x * Int63.wB) mod 2 ^ 64 = if Z.odd x then Int63.wB else 0.
+Proof.
+remember (Z.odd x) as last_bit.
+rewrite (Zdiv2_odd_eqn x). subst.
+rewrite Z.mul_add_distr_r.
+replace (2 * Z.div2 x) with (Z.div2 x * 2) by apply Z.mul_comm.
+rewrite<- Z.mul_assoc.
+replace (2 * Int63.wB) with (2 ^ 64)%Z by trivial.
+rewrite Z.add_comm. rewrite Z.mod_add by discriminate.
+now destruct (Z.odd x).
+Qed.
+
+Lemma add_ok (a b: uint64):
+  Z_of_uint64 (add a b) = ((Z_of_uint64 a + Z_of_uint64 b) mod 2^64).
+Proof.
+assert (L := Z_of_uint64_lower (add a b)).
+assert (U := Z_of_uint64_upper (add a b)).
+repeat rewrite<- Z_of_uint64_alt in *.
+rewrite<- (Z.mod_small (Z_of_uint64' (add a b)) (2 ^ 64)) by tauto.
+unfold add. destruct a as (ha, la). destruct b as (hb, lb).
+assert (R := Int63.addc_spec la lb).
+cbn in L. cbn in U.
+unfold DoubleType.interp_carry in R.
+remember (Int63.addc la lb) as x. clear Heqx.
+unfold Z_of_uint64'.
+destruct x; 
+  [rewrite R | try rewrite Z.mul_1_l in R;
+               replace (Int63.to_Z i) with (Int63.to_Z la + Int63.to_Z lb + (-1) * Int63.wB) by lia];
+  wB_up; wB_up; repeat rewrite<- Z.add_assoc;
+  apply Z_mod_add_r;
+  destruct ha, hb; rewrite mod_wB; trivial.
+Qed.
+
+(*******************************************************************************)
+
+Definition shr_uint63 (a: uint64) (sh: uint63)
+: uint64
+:= if (sh == 0)%int63
+     then a
+     else let (hi, lo) := a in
+       (false, if hi
+                 then (((1 << 62) >> (sh - 1)) lor (lo >> sh))%int63
+                 else lsr lo sh).
+
+Lemma shr_uint63_ok (a: uint64) (sh: uint63):
+  Z_of_uint64 (shr_uint63 a sh) = Z.shiftr (Z_of_uint64 a) (Int63.to_Z sh).
+Proof.
+unfold shr_uint63.
+remember ((sh == 0)%int63) as sh0 eqn:Sh0. symmetry in Sh0. destruct sh0.
+{ rewrite Int63.eqb_spec in Sh0. now subst. }
+assert(BS := to_Z_bounded sh). remember (to_Z sh) as s.
+assert(SPos: 0 < s).
+{
+  enough (s <> 0) by lia.
+  intro H. subst.
+  replace 0 with (to_Z 0) in H by trivial.
+  apply to_Z_inj in H.
+  apply eqb_spec in H.
+  rewrite H in Sh0.
+  discriminate.
+}
+destruct a as (hi, lo).
+destruct hi; unfold Z_of_uint64.
+2:{
+  (* low case *)
+  rewrite Int63.lsr_spec.
+  rewrite Z.shiftr_div_pow2 by tauto.
+  now subst.
+}
+(* high case *)
+rewrite Int63.lor_spec'.
+rewrite Int63.lsr_spec.
+rewrite Int63.lsr_spec.
+rewrite Int63.lsl_spec.
+rewrite Int63.sub_spec.
+replace (to_Z 1) with 1 by trivial.
+replace (to_Z 62) with 62 by trivial.
+rewrite<- Heqs.
+clear Sh0 Heqs.
+assert(BN := to_Z_bounded lo). remember (to_Z lo) as n. clear Heqn.
+rewrite Z.mul_1_l. rewrite Z.shiftr_div_pow2 by tauto.
+replace (2 ^ 62 mod wB) with (2 ^ 62) by trivial.
+replace ((s - 1) mod wB) with (s - 1). 2:{ symmetry. apply Z.mod_small. lia. }
+assert (CS: 64 <= s \/ s <= 63) by lia.
+case CS; clear CS; intro CS.
+{
+  (* large shift, everything is 0 *)
+  replace (n / 2 ^ s) with 0.
+  2:{
+    symmetry. apply Z.div_small.
+    split. { tauto. }
+    replace Int63.wB with (2 ^ 63) in * by trivial.
+    apply (Z.lt_trans n (2^63) (2^s)). { tauto. }
+    apply Z.pow_lt_mono_r; lia.
+  }
+  rewrite Z.lor_0_r. 
+  rewrite Z.div_small.
+  2:{
+    split. { lia. }
+    apply Z.pow_lt_mono_r; lia.
+  }
+  rewrite Z.div_small. { trivial. }
+  split. { lia. }
+  apply (Z.lt_le_trans _ (2^64) (2^s)).
+  { replace (2 ^ 64) with (wB + wB) by trivial. lia. }
+  apply Z.pow_le_mono_r; lia.
+}
+replace (2 ^ 62 / 2 ^ (s - 1)) with (2 ^ 63 / 2 ^ s). 
+2:{
+  replace (2 ^ 63) with (2 * (2 ^ 62)) by trivial.
+  replace (2 ^ s) with ((2 ^ (1 + (s - 1)))) by now replace (1 + (s - 1)) with s by lia.
+  rewrite Z.pow_add_r; try lia.
+  rewrite Z.div_mul_cancel_l; try lia.
+  apply Z.pow_nonzero; lia.
+}
+repeat rewrite<- Z.shiftr_div_pow2 by tauto.
+rewrite<- Z.shiftr_lor.
+f_equal.
+rewrite<- Arith2.Z_add_nocarry_lor. { apply Z.add_comm. }
+rewrite Z.land_comm.
+apply Arith2.Z_land_pow2_small. { tauto. }
+now rewrite<- Z.leb_le.
+Qed.
+
+(*******************************************************************************)
+
+Definition shl_uint63 (a: uint64) (sh: uint63)
+: uint64
+:= if (sh == 0)%int63
+     then a
+     else let (hi, lo) := a in
+       (get_digit lo (63 - sh), lsl lo sh).
+
+Lemma shl_uint63_ok (a: uint64) (sh: uint63):
+  Z_of_uint64 (shl_uint63 a sh) = (Z.shiftl (Z_of_uint64 a) (Int63.to_Z sh) mod 2^64)%Z.
+Proof.
+repeat rewrite<- Z_of_uint64_alt. repeat rewrite<- Z_of_uint64_lor'_ok.
+unfold shl_uint63.
+remember ((sh == 0)%int63) as sh0 eqn:Sh0. symmetry in Sh0. destruct sh0.
+{ 
+  rewrite Int63.eqb_spec in Sh0. subst. rewrite Z.shiftl_0_r.
+  symmetry. apply Z.mod_small.
+  rewrite Z_of_uint64_lor'_ok.
+  rewrite Z_of_uint64_alt.
+  split. { apply Z_of_uint64_lower. } apply Z_of_uint64_upper.
+}
+assert(BS := to_Z_bounded sh). remember (to_Z sh) as s.
+assert(SPos: 0 < s).
+{
+  enough (s <> 0) by lia.
+  intro H. subst.
+  replace 0 with (to_Z 0) in H by trivial.
+  apply to_Z_inj in H.
+  apply eqb_spec in H.
+  rewrite H in Sh0.
+  discriminate.
+}
+destruct a as (hi, lo).
+rewrite uint63_testbit_Z.
+unfold Z_of_uint64_lor'.
+rewrite Int63.lsl_spec.
+apply Z.bits_inj'. intros k Knonneg.
+rewrite Z.lor_spec.
+rewrite<- Z.shiftl_mul_pow2 by now subst.
+rewrite<- Heqs.
+assert (BN := to_Z_bounded lo). remember (to_Z lo) as n.
+rewrite Z.shiftl_lor.
+replace wB with (2^63) by trivial.
+repeat rewrite<- Z.land_ones.
+rewrite Z.land_lor_distr_l.
+replace (Z.land (Z.shiftl ((if hi then 1 else 0) * 2 ^ 63) s) (Z.ones 64)) with 0.
+3-4: now rewrite<- Z.leb_le.
+2:{
+  destruct hi. 2:{ rewrite Z.mul_0_l. rewrite Z.shiftl_0_l. rewrite Z.land_0_l. trivial. }
+  symmetry.
+  rewrite Z.mul_1_l.
+  rewrite Z.shiftl_mul_pow2 by tauto.
+  rewrite Z.land_ones by now rewrite<- Z.leb_le.
+  rewrite<- Z.pow_add_r; try lia.
+  replace (2 ^ (63 + s)) with (2^(s - 1) * 2^64).
+  2:{ rewrite<- Z.pow_add_r; try f_equal; lia. }
+  apply Z_mod_mult.
+}
+rewrite Z.lor_0_r.
+repeat rewrite Z.land_spec.
+repeat rewrite Z.testbit_ones_nonneg; try lia.
+remember (Z.testbit (Z.shiftl n s) k) as x.
+assert (CK: k <> 63 \/ k = 63) by lia.
+case CK; clear CK; intro CK.
+{
+  replace (Z.testbit ((if Z.testbit n (to_Z (63 - sh)%int63) then 1 else 0) * 2 ^ 63) k) with false.
+  2:{
+    symmetry.
+    destruct (Z.testbit n (to_Z (63 - sh)%int63)); [ rewrite Z.mul_1_l | rewrite Z.mul_0_l ].
+    { apply Z.pow2_bits_false. lia. }
+    apply Z.bits_0.
+  }
+  rewrite Bool.orb_false_r.
+  f_equal.
+  rewrite Arith2.Z_ltb_lt_quad. split; lia.
+}
+subst k x.
+replace (63 <? 63) with false by trivial.
+replace (63 <? 64) with true by trivial.
+rewrite Bool.andb_false_r. rewrite Bool.orb_false_l. rewrite Bool.andb_true_r.
+rewrite Arith2.Z_testbit_flag_mul_pow2 by lia.
+rewrite Z.shiftl_spec by lia.
+rewrite sub_spec. replace (to_Z 63) with 63 by trivial.
+rewrite<- Heqs.
+assert (WB63: 63 < wB) by now rewrite<- Z.ltb_lt.
+assert (Q: (63 - s) mod wB = 63 - s \/ 63 < (63 - s) mod wB).
+{
+  assert(B: -wB < 63 - s) by lia.
+  assert(WBNZ: wB <> 0) by discriminate.
+  assert(D := Z.div_mod (63 - s) wB WBNZ).
+  assert(WBPos: 0 < wB) by lia.
+  assert(BQ := Z.mod_pos_bound (63 - s) wB WBPos).
+  remember ((63 - s) mod wB) as q.
+  clear Heqq.
+  assert (L: -1 <= (63 - s) / wB) by nia.
+  assert (U: (63 - s) / wB <= 0) by nia.
+  assert (T: (63 - s) / wB = 0 \/ (63 - s) / wB = -1) by lia.
+  case T; clear T; intro T; lia.
+}
+case Q; clear Q; intro Q. { now rewrite Q. }
+assert (S63: 63 < s).
+{
+  apply Z.nle_gt. intro H.
+  replace ((63 - s) mod wB) with (63 - s) in *. 
+  2:{ 
+    rewrite Z.mod_small. { trivial. } 
+    lia.
+  }
+  lia.
+}
+rewrite (Z.testbit_neg_r n (63 - s)) by lia.
+apply Arith2.Z_testbit_small. { tauto. }
+refine (Z.lt_trans n wB _ _ _). { tauto. }
+replace wB with (2^63) by trivial.
+apply Z.pow_lt_mono_r; try lia.
+apply Z.mod_pos_bound.
+trivial. apply Q.
+Qed.
+
+(*******************************************************************************)
+
+Definition bitwise_or (a b: uint64)
+: uint64
+:= ((fst a || fst b)%bool,  Int63.lor (snd a) (snd b)).
+
+Lemma bitwise_or_ok (a b: uint64):
+  Z_of_uint64 (bitwise_or a b) = (Z.lor (Z_of_uint64 a) (Z_of_uint64 b)).
+Proof.
+repeat rewrite<- Z_of_uint64_lor_ok.
+destruct a as (a_hi, a_lo).
+destruct b as (b_hi, b_lo).
+unfold Z_of_uint64_lor. unfold bitwise_or.
+destruct a_hi, b_hi;
+  match goal with
+  |- (if ?cond then _ else _) = ?rhs  => remember cond as c; cbn in Heqc; subst
+  end;
+  repeat rewrite lor_spec';
+  replace (snd (_, a_lo)) with a_lo by trivial;
+  replace (snd (_, b_lo)) with b_lo by trivial;
+  remember (to_Z a_lo) as x;
+  remember (to_Z b_lo) as y;
+  repeat rewrite Z.lor_assoc; trivial.
+{
+  (* goal: Z.lor (Z.lor x y) wB = Z.lor (Z.lor (Z.lor x wB) y) wB *)
+  repeat rewrite<- Z.lor_assoc. f_equal.
+  rewrite Z.lor_comm.
+  rewrite Z.lor_assoc.
+  now replace (Z.lor wB wB) with wB by trivial.
+}
+(* goal: Z.lor (Z.lor x y) wB = Z.lor (Z.lor x wB) y *)
+repeat rewrite<- Z.lor_assoc. f_equal.
+apply Z.lor_comm.
+Qed.
+
+(*******************************************************************************)
+
+Definition bitwise_xor (a b: uint64)
+: uint64
+:= (xorb (fst a) (fst b),  Int63.lxor (snd a) (snd b)).
+
+Lemma bitwise_xor_ok (a b: uint64):
+  Z_of_uint64 (bitwise_xor a b) = (Z.lxor (Z_of_uint64 a) (Z_of_uint64 b)).
+Proof.
+repeat rewrite<- Z_of_uint64_lxor_ok.
+destruct a as (a_hi, a_lo).
+destruct b as (b_hi, b_lo).
+unfold Z_of_uint64_lxor. unfold bitwise_xor.
+destruct a_hi, b_hi;
+  match goal with
+  |- (if ?cond then _ else _) = ?rhs  => remember cond as c; cbn in Heqc; subst
+  end;
+  repeat rewrite lxor_spec';
+  replace (snd (_, a_lo)) with a_lo by trivial;
+  replace (snd (_, b_lo)) with b_lo by trivial;
+  remember (to_Z a_lo) as x;
+  remember (to_Z b_lo) as y; 
+  repeat rewrite Z.lxor_assoc; trivial.
+{
+  (* goal: Z.lxor x y = Z.lxor x (Z.lxor wB (Z.lxor y wB)) *)
+  rewrite (Z.lxor_comm y wB). f_equal.
+  rewrite<- Z.lxor_assoc.
+  now replace (Z.lor wB wB) with wB by trivial.
+}
+f_equal. apply Z.lxor_comm.
+Qed.
+
+(*******************************************************************************)
+
+Definition bitwise_and (a b: uint64)
+: uint64
+:= ((fst a && fst b)%bool,  Int63.land (snd a) (snd b)).
+
+Lemma bitwise_and_ok (a b: uint64):
+  Z_of_uint64 (bitwise_and a b) = (Z.land (Z_of_uint64 a) (Z_of_uint64 b)).
+Proof.
+repeat rewrite<- Z_of_uint64_lor_ok.
+destruct a as (a_hi, a_lo).
+destruct b as (b_hi, b_lo).
+unfold Z_of_uint64_lor. unfold bitwise_and.
+destruct a_hi, b_hi;
+  match goal with
+  |- (if ?cond then _ else _) = ?rhs  => remember cond as c; cbn in Heqc; subst
+  end;
+  repeat rewrite land_spec';
+  replace (snd (_, a_lo)) with a_lo by trivial;
+  replace (snd (_, b_lo)) with b_lo by trivial;
+  remember (to_Z a_lo) as x;
+  remember (to_Z b_lo) as y;
+  repeat rewrite Z.land_assoc; trivial.
+{ apply Z.lor_land_distr_l. }
+{ 
+  rewrite Z.land_lor_distr_l.
+  replace (Z.land wB y) with 0. { now rewrite Z.lor_0_r. }
+  symmetry. rewrite Z.land_comm. apply Arith2.Z_land_pow2_small.
+  { subst. apply to_Z_bounded. }
+  rewrite<- Z.leb_le. trivial.
+}
+rewrite Z.land_lor_distr_r.
+replace (Z.land x wB) with 0. { now rewrite Z.lor_0_r. }
+symmetry. apply Arith2.Z_land_pow2_small.
+{ subst. apply to_Z_bounded. }
+rewrite<- Z.leb_le. trivial.
+Qed.
+
+(*******************************************************************************)
+
+Definition bitwise_not (a: uint64)
+: uint64
+:= (negb (fst a),  Int63.lxor (snd a) (of_Z (-1))).
+
+Lemma bitwise_not_via_xor (a: uint64):
+  bitwise_not a = bitwise_xor a uint64_max_value.
+Proof.
+trivial.
+Qed.
+
+Lemma bitwise_not_ok (a: uint64):
+  Z_of_uint64 (bitwise_not a) = (Z.lnot (Z_of_uint64 a)) mod 2^64.
+Proof.
+rewrite bitwise_not_via_xor. rewrite bitwise_xor_ok.
+rewrite<- Z.lxor_m1_r. rewrite<- Z.land_ones. 2: { now rewrite<- Z.leb_le. }
+assert (L := Z_of_uint64_lower a).
+assert (U := Z_of_uint64_upper a).
+remember (Z_of_uint64 a) as x. clear Heqx.
+rewrite uint64_max_value_ok.
+replace (2 ^ 64 - 1) with (Z.ones 64) by trivial.
+rewrite Z_land_lxor_distr_l.
+f_equal.
+symmetry. apply Z.land_ones_low. { assumption. }
+apply Arith2.Z_log2_lt_pow2; try assumption.
+now rewrite<- Z.ltb_lt.
+Qed.
+
+(*******************************************************************************)
+
+Definition uint64_of_be_bytes (b: byte * byte * byte * byte * byte * byte * byte * byte)
+: uint64
+:= match b with
+   | (b7, b6, b5, b4, b3, b2, b1, b0) =>
+       bitwise_or (shl_uint63 (false, int_of_byte b7) 56%int63)
+                  (false, ((int_of_byte b6 << 48) lor (int_of_byte b5 << 40) lor (int_of_byte b4 << 32)
+                       lor (int_of_byte b3 << 24) lor (int_of_byte b2 << 16) lor (int_of_byte b1 << 8)
+                       lor int_of_byte b0)%int63)
+   end.
+
+Definition uint64_to_be_bytes (a: uint64)
+: byte * byte * byte * byte * byte * byte * byte * byte
+:= let (f, i) := a in
+    (byte_of_int (snd (shr_uint63 a 56)),
+     byte_of_int (i >> 48),
+     byte_of_int (i >> 40),
+     byte_of_int (i >> 32),
+     byte_of_int (i >> 24),
+     byte_of_int (i >> 16),
+     byte_of_int (i >> 8),
+     byte_of_int i)%int63.
+
+Definition uint64_to_le_bytes (a: uint64)
+: byte * byte * byte * byte * byte * byte * byte * byte
+:= let (f, i) := a in
+    (byte_of_int i,
+     byte_of_int (i >> 8),
+     byte_of_int (i >> 16),
+     byte_of_int (i >> 24),
+     byte_of_int (i >> 32),
+     byte_of_int (i >> 40),
+     byte_of_int (i >> 48),
+     byte_of_int (snd (shr_uint63 a 56)))%int63.
+
+
+(*******************************************************************************)
+
+Definition uint64_of_N_divmod (n: N)
+: N * uint64
+:= (N.shiftr n 64, (N.testbit n 63, Int63.of_Z (Z.of_N n))).
+
+Definition uint64_of_pos_divmod (p: positive)
+: N * uint64
+:= uint64_of_N_divmod (N.pos p).
+
+Definition head0 (a: uint64)
+: int
+:= let (hi, lo) := a in
+   if hi
+     then 0
+     else succ (head0 lo).
+
+Definition head0_uint64 (a: uint64)
+: uint64
+:= (false, head0 a).
+
+Definition tail0 (a: uint64)
+: int
+:= let (hi, lo) := a in
+   if eqb lo 0
+     then if hi then 63 else 64
+     else tail0 lo.
+
+Definition tail0_uint64 (a: uint64)
+: uint64
+:= (false, tail0 a).
+
+Definition compare (a b: uint64)
+: comparison
+:= match a, b with
+   | (true, x), (true, y) | (false, x), (false, y) => compare x y
+   | (true, _), (false, _) => Gt
+   | (false, _), (true, _) => Lt
+   end.
+
+Definition eq0 (a: uint64)
+: bool
+:= let (hi, lo) := a in
+   if hi
+     then false
+     else eqb lo 0%int63.
+
+Definition succ (a: uint64)
+: uint64
+:= let (hi, lo) := a in
+   match succc lo with
+   | C0 n => (hi, n)
+   | C1 n => (negb hi, n)
+   end.
