L10/UInt256.v
@@ -1,29 +1,66 @@
 From Coq Require Import ZArith.
 Require Import Config L10.AST.
 
+(** Bitwise not *)
+Definition uint256_not {C: VyperConfig} (a: uint256)
+:= uint256_of_Z (Z.lxor (Z.ones 256) (Z_of_uint256 a)).
+
+(** Logical not ("iszero"). *)
+Definition uint256_iszero {C: VyperConfig} (a: uint256)
+:= if (Z_of_uint256 a =? 0)%Z
+     then one256
+     else zero256.
+
 Definition interpret_unop {C: VyperConfig} (op: unop) (a: uint256)
 : option uint256
 := match op with
-   | BitwiseNot => Some (uint256_of_Z (Z.lxor (Z.ones 256) (Z_of_uint256 a)))
+   | BitwiseNot => Some (uint256_not a)
    | Neg => maybe_uint256_of_Z (- Z_of_uint256 a) (* This only allows 0. *)
-   | LogicalNot => let az := Z_of_uint256 a in
-                   Some (if (az =? 0)%Z
-                          then one256
-                          else zero256)
+   | LogicalNot => Some (uint256_iszero a)
    end.
+
+(** Bitwise and *)
+Definition uint256_and {C: VyperConfig} (a b: uint256)
+:= uint256_of_Z (Z.land (Z_of_uint256 a) (Z_of_uint256 b)).
+
+(** Bitwise or *)
+Definition uint256_or {C: VyperConfig} (a b: uint256)
+:= uint256_of_Z (Z.lor (Z_of_uint256 a) (Z_of_uint256 b)).
+
+(** Bitwise xor *)
+Definition uint256_xor {C: VyperConfig} (a b: uint256)
+:= uint256_of_Z (Z.lxor (Z_of_uint256 a) (Z_of_uint256 b)).
+
+Definition uint256_lt {C: VyperConfig} (a b: uint256)
+:= if (Z_of_uint256 a <?  Z_of_uint256 b)%Z then one256 else zero256.
+
+Definition uint256_eq {C: VyperConfig} (a b: uint256)
+:= if (Z_of_uint256 a =?  Z_of_uint256 b)%Z then one256 else zero256.
+
+Definition uint256_gt {C: VyperConfig} (a b: uint256)
+:= if (Z_of_uint256 a >?  Z_of_uint256 b)%Z then one256 else zero256.
+
+Definition uint256_le {C: VyperConfig} (a b: uint256)
+:= if (Z_of_uint256 a <=?  Z_of_uint256 b)%Z then one256 else zero256.
+
+Definition uint256_ge {C: VyperConfig} (a b: uint256)
+:= if (Z_of_uint256 a >=?  Z_of_uint256 b)%Z then one256 else zero256.
+
+Definition uint256_ne {C: VyperConfig} (a b: uint256)
+:= if (Z_of_uint256 a =?  Z_of_uint256 b)%Z then zero256 else one256.
 
 Definition interpret_binop {C: VyperConfig} (op: binop) (a b: uint256)
 : option uint256
 := match op with
-   | Lt => Some (if (Z_of_uint256 a <?  Z_of_uint256 b)%Z then one256 else zero256)
-   | Le => Some (if (Z_of_uint256 a <=? Z_of_uint256 b)%Z then one256 else zero256)
-   | Gt => Some (if (Z_of_uint256 a >?  Z_of_uint256 b)%Z then one256 else zero256)
-   | Ge => Some (if (Z_of_uint256 a >=? Z_of_uint256 b)%Z then one256 else zero256)
-   | Eq => Some (if (Z_of_uint256 a =?  Z_of_uint256 b)%Z then one256 else zero256)
-   | Ne => Some (if (Z_of_uint256 a =?  Z_of_uint256 b)%Z then zero256 else one256)
-   | BitwiseOr  => Some (uint256_of_Z (Z.lor  (Z_of_uint256 a) (Z_of_uint256 b)))
-   | BitwiseAnd => Some (uint256_of_Z (Z.land (Z_of_uint256 a) (Z_of_uint256 b)))
-   | BitwiseXor => Some (uint256_of_Z (Z.lxor (Z_of_uint256 a) (Z_of_uint256 b)))
+   | Lt => Some (uint256_lt a b)
+   | Le => Some (uint256_le a b)
+   | Gt => Some (uint256_gt a b)
+   | Ge => Some (uint256_ge a b)
+   | Eq => Some (uint256_eq a b)
+   | Ne => Some (uint256_ne a b)
+   | BitwiseOr  => Some (uint256_or a b)
+   | BitwiseAnd => Some (uint256_and a b)
+   | BitwiseXor => Some (uint256_xor a b)
    (* Nov 2020: changed shifts to checked as x << n is basically arithmetic, namely x * 2**n *)
    | ShiftLeft  => maybe_uint256_of_Z (Z.shiftl (Z_of_uint256 a) (Z_of_uint256 b))
    | ShiftRight => maybe_uint256_of_Z (Z.shiftr (Z_of_uint256 a) (Z_of_uint256 b))
