L30/VarCap.v
@@ -1,0 +1,41 @@
+From Coq Require Import NArith.
+
+From Vyper Require Import Config.
+From Vyper.L30 Require Import AST.
+
+Definition var_cap_small_stmt {C: VyperConfig} (ss: small_stmt)
+: N
+:= match ss with
+   | Pass => 0
+   | Const dst _ => N.succ dst
+   | Copy dst src => N.succ (N.max dst src)
+   | StorageGet dst _ => N.succ dst
+   | StoragePut _ src => N.succ src
+   | UnOp _ dst src => N.succ (N.max dst src)
+   | PowConstBase dst base exp => N.succ (N.max dst exp)
+   | PowConstExp  dst base exp => N.succ (N.max dst base)
+   | BinOp _ dst src1 src2 _ => N.succ (N.max dst (N.max src1 src2))
+   | PrivateCall dst _ offset count | BuiltinCall dst _ offset count =>
+      match count with
+      | 0%N => N.succ dst
+      | _ => N.max (N.succ dst) (offset + count)%N
+      end
+   | Abort _ => 0
+   | Return src => N.succ src
+   | Raise src => N.succ src
+   end.
+
+Fixpoint var_cap_stmt {C: VyperConfig} (s: stmt)
+:= match s with
+   | SmallStmt ss => var_cap_small_stmt ss
+   | IfElseStmt cond_src yes no =>
+        N.max (N.succ cond_src) (N.max (var_cap_stmt yes) (var_cap_stmt no))
+   | Loop var _ body => N.max (N.succ var) (var_cap_stmt body)
+   | Semicolon a b => N.max (var_cap_stmt a) (var_cap_stmt b)
+   end.
+
+Fixpoint var_cap_decl {C: VyperConfig} (d: decl)
+:= match d with
+   | StorageVarDecl _ => 0%N
+   | FunDecl _ args_count body => N.max args_count (var_cap_stmt body)
+   end.
