Lib2/Arith2.v
@@ -1,0 +1,531 @@
+From Coq Require Import NArith ZArith Lia.
+
+From Vyper Require Import Logic2.
+
+(**************************************************************************)
+
+Lemma N_ltb_lt_quad (a b c d: N):
+  ((a <? b)%N = (c <? d)%N) <-> ((a < b)%N <-> (c < d)%N).
+Proof.
+apply relation_quad; apply N.ltb_lt.
+Qed.
+
+Lemma Z_ltb_lt_quad (a b c d: Z):
+  ((a <? b)%Z = (c <? d)%Z) <-> ((a < b)%Z <-> (c < d)%Z).
+Proof.
+apply relation_quad; apply Z.ltb_lt.
+Qed.
+
+Lemma N_leb_le_quad (a b c d: N):
+  ((a <=? b)%N = (c <=? d)%N) <-> ((a <= b)%N <-> (c <= d)%N).
+Proof.
+apply relation_quad; apply N.leb_le.
+Qed.
+
+Lemma Z_leb_le_quad (a b c d: Z):
+  ((a <=? b)%Z = (c <=? d)%Z) <-> ((a <= b)%Z <-> (c <= d)%Z).
+Proof.
+apply relation_quad; apply Z.leb_le.
+Qed.
+
+Lemma N2Z_ltb (n m: N):
+  (n <? m)%N = (Z.of_N n <? Z.of_N m)%Z.
+Proof.
+apply (relation_quad N.ltb_lt Z.ltb_lt).
+apply N2Z.inj_lt.
+Qed.
+
+Lemma N2Z_leb (n m: N):
+  (n <=? m)%N = (Z.of_N n <=? Z.of_N m)%Z.
+Proof.
+apply (relation_quad N.leb_le Z.leb_le).
+apply N2Z.inj_le.
+Qed.
+
+(**************************************************************************)
+
+Lemma Z_shiftr_pow2 (n: Z) (B: (0 <= n)%Z):
+  Z.shiftr (2 ^ n) n = 1%Z.
+Proof.
+rewrite (Z.shiftr_div_pow2 _ _ B).
+apply Z.div_same.
+now apply Z.pow_nonzero.
+Qed.
+
+Lemma Z_ltb_irrefl (n: Z):
+  (n <? n)%Z = false.
+Proof.
+remember (n <? n)%Z as L.
+destruct L; trivial.
+symmetry in HeqL.
+rewrite Z.ltb_lt in HeqL.
+apply Z.lt_irrefl in HeqL.
+contradiction.
+Qed.
+
+Lemma N_ltb_irrefl (n: N):
+  (n <? n)%N = false.
+Proof.
+remember (n <? n)%N as L.
+destruct L; trivial.
+symmetry in HeqL.
+rewrite N.ltb_lt in HeqL.
+apply N.lt_irrefl in HeqL.
+contradiction.
+Qed.
+
+(**************************************************************************)
+
+Lemma Z_land_pow2_shift (n m: Z) (BM: (0 <= m)%Z):
+  Z.land n (2 ^ m) = Z.shiftl (Z.land (Z.shiftr n m) 1) m.
+Proof.
+rewrite<- (Z_shiftr_pow2 m BM).
+rewrite<- Z.shiftr_land.
+rewrite<- (Z.ldiff_ones_r _ _ BM).
+rewrite Z.ldiff_land.
+rewrite<- Z.land_assoc.
+f_equal.
+apply Z.bits_inj'. intros k Bk.
+rewrite Z.land_spec.
+rewrite (Z.lnot_spec _ _ Bk).
+rewrite (Z.testbit_ones _ _ BM).
+rewrite (Z.pow2_bits_eqb _ _ BM).
+rewrite<- Z.leb_le in Bk.
+rewrite Bk.
+rewrite Bool.andb_true_l.
+remember (m =? k)%Z as MK. symmetry in HeqMK.
+destruct MK. 
+{
+  rewrite Z.eqb_eq in HeqMK. subst.
+  now rewrite Z_ltb_irrefl.
+}
+trivial.
+Qed.
+
+Lemma Z_mul_pos_iff_l (n m: Z) (BM: (0 < m)%Z):
+  (0 < n)%Z <-> (0 < n * m)%Z.
+Proof.
+split. { intro. apply Z.mul_pos_pos; assumption. }
+apply (Z.mul_pos_cancel_r _ _ BM).
+Qed.
+
+Lemma Z_mul_pos_iff_r (n m: Z) (BN: (0 < n)%Z):
+  (0 < m)%Z <-> (0 < n * m)%Z.
+Proof.
+split. { apply (Z.mul_pos_pos _ _ BN). }
+apply (Z.mul_pos_cancel_l _ _ BN).
+Qed.
+
+Lemma Z_shiftl_pos_iff (n m: Z) (BM: (0 <= m)%Z):
+ (0 < n)%Z <-> (0 < Z.shiftl n m)%Z.
+Proof.
+rewrite (Z.shiftl_mul_pow2 _ _ BM).
+apply Z_mul_pos_iff_l.
+apply Z.pow_pos_nonneg.
+{ rewrite<- Z.ltb_lt. trivial. }
+assumption.
+Qed.
+
+Lemma Z_odd_land_1 (n: Z) (B: (0 <= n)%Z):
+  Z.odd n = (0 <? Z.land n 1)%Z.
+Proof.
+destruct n; now try destruct p.
+Qed.
+
+Lemma Z_testbit_alt (n m: Z) (BN: (0 <= n)%Z) (BM: (0 <= m)%Z):
+  Z.testbit n m = (0 <? Z.land n (2 ^ m))%Z.
+Proof.
+rewrite (Z_land_pow2_shift _ _ BM).
+assert (Q: forall x, ((0 <? Z.shiftl x m) = (0 <? x))%Z).
+{
+  intro x.
+  rewrite Z_ltb_lt_quad.
+  symmetry.
+  apply Z_shiftl_pos_iff.
+  assumption.
+}
+rewrite Q. clear Q.
+rewrite Z.testbit_odd.
+apply Z_odd_land_1.
+apply Z.shiftr_nonneg.
+assumption.
+Qed.
+
+Lemma Z_testbit_high (a n: Z)
+                      (B: (0 <= n)%Z)
+                      (A: (0 <= a < 2 ^ n)%Z):
+  Z.testbit a n = false.
+Proof.
+rewrite<- (Z.mod_small a (2 ^ n)%Z A).
+apply Z.mod_pow2_bits_high.
+split. { assumption. }
+apply Z.le_refl.
+Qed.
+
+(**************************************************************************)
+
+Lemma Z_to_N_land (x y: Z) (BX: (0 <= x)%Z) (BY: (0 <= y)%Z):
+  Z.to_N (Z.land x y) = N.land (Z.to_N x) (Z.to_N y).
+Proof.
+apply N.bits_inj. intro n.
+rewrite N.land_spec.
+remember (Z.of_N n) as m.
+assert (NM: n = Z.to_N m).
+{ subst m. symmetry. apply N2Z.id. }
+repeat rewrite NM.
+assert (BM: (0 <= m)%Z).
+{ subst. apply N2Z.is_nonneg. }
+repeat rewrite<- Z2N.inj_testbit; try assumption.
+repeat rewrite Z2N.id; try assumption.
+{ apply Z.land_spec. }
+rewrite Z.land_nonneg. tauto.
+Qed.
+
+
+Lemma N_to_Z_land (x y: N):
+  Z.of_N (N.land x y) = Z.land (Z.of_N x) (Z.of_N y).
+Proof.
+rewrite<- (Z2N.id (Z.land (Z.of_N x) (Z.of_N y))).
+{
+  f_equal.
+  rewrite Z_to_N_land; try apply N2Z.is_nonneg.
+  repeat rewrite N2Z.id.
+  trivial.
+}
+apply Z.land_nonneg. left. apply N2Z.is_nonneg.
+Qed.
+
+Lemma Z_to_N_lor (x y: Z) (BX: (0 <= x)%Z) (BY: (0 <= y)%Z):
+  Z.to_N (Z.lor x y) = N.lor (Z.to_N x) (Z.to_N y).
+Proof.
+apply N.bits_inj. intro n.
+rewrite N.lor_spec.
+remember (Z.of_N n) as m.
+assert (NM: n = Z.to_N m).
+{ subst m. symmetry. apply N2Z.id. }
+repeat rewrite NM.
+assert (BM: (0 <= m)%Z).
+{ subst. apply N2Z.is_nonneg. }
+repeat rewrite<- Z2N.inj_testbit; try assumption.
+repeat rewrite Z2N.id; try assumption.
+{ apply Z.lor_spec. }
+rewrite Z.lor_nonneg. tauto.
+Qed.
+
+Lemma N_to_Z_lor (x y: N):
+  Z.of_N (N.lor x y) = Z.lor (Z.of_N x) (Z.of_N y).
+Proof.
+rewrite<- (Z2N.id (Z.lor (Z.of_N x) (Z.of_N y))).
+{
+  f_equal.
+  rewrite Z_to_N_lor; try apply N2Z.is_nonneg.
+  repeat rewrite N2Z.id.
+  trivial.
+}
+apply Z.lor_nonneg. split; apply N2Z.is_nonneg.
+Qed.
+
+Lemma Z_to_N_lxor (x y: Z) (BX: (0 <= x)%Z) (BY: (0 <= y)%Z):
+  Z.to_N (Z.lxor x y) = N.lxor (Z.to_N x) (Z.to_N y).
+Proof.
+apply N.bits_inj. intro n.
+rewrite N.lxor_spec.
+remember (Z.of_N n) as m.
+assert (NM: n = Z.to_N m).
+{ subst m. symmetry. apply N2Z.id. }
+repeat rewrite NM.
+assert (BM: (0 <= m)%Z).
+{ subst. apply N2Z.is_nonneg. }
+repeat rewrite<- Z2N.inj_testbit; try assumption.
+repeat rewrite Z2N.id; try assumption.
+{ apply Z.lxor_spec. }
+rewrite Z.lxor_nonneg. tauto.
+Qed.
+
+Lemma N_to_Z_lxor (x y: N):
+  Z.of_N (N.lxor x y) = Z.lxor (Z.of_N x) (Z.of_N y).
+Proof.
+rewrite<- (Z2N.id (Z.lxor (Z.of_N x) (Z.of_N y))).
+{
+  f_equal.
+  rewrite Z_to_N_lxor; try apply N2Z.is_nonneg.
+  repeat rewrite N2Z.id.
+  trivial.
+}
+apply Z.lxor_nonneg. split; intro; apply N2Z.is_nonneg.
+Qed.
+
+(**************************************************************************)
+
+Lemma N_testbit_alt (n m: N):
+  N.testbit n m = (0 <? N.land n (2 ^ m))%N.
+Proof.
+rewrite<- Z.testbit_of_N.
+replace (0 <? N.land n (2 ^ m))%N with (0 <? Z.land (Z.of_N n) (2 ^ (Z.of_N m)))%Z.
+2:{
+  rewrite N2Z_ltb.
+  rewrite N_to_Z_land.
+  cbn.
+  repeat f_equal.
+  rewrite N2Z.inj_pow.
+  trivial.
+}
+apply Z_testbit_alt; apply N2Z.is_nonneg.
+Qed.
+
+(**************************************************************************)
+
+Definition N_0_lt_pow2 (n: N):
+  (0 < 2 ^ n)%N.
+Proof.
+case (N.eq_0_gt_0_cases (2 ^ n)); intro; try assumption.
+apply N.pow_nonzero in H. { contradiction. }
+discriminate.
+Qed.
+
+Definition Z_0_lt_pow2 (n: Z) (B: (0 <= n)%Z):
+  (0 < 2 ^ n)%Z.
+Proof.
+assert (A := N_0_lt_pow2 (Z.to_N n)).
+apply N2Z.inj_lt in A.
+rewrite N2Z.inj_pow in A.
+cbn in A.
+now rewrite Z2N.id in A.
+Qed.
+
+Lemma N_ne_0_gt_0 (n: N):
+  n <> 0%N <-> (0 < n)%N.
+Proof.
+split; intro H.
+{ assert (CN := N.eq_0_gt_0_cases n). tauto. }
+destruct n. { now apply N.lt_irrefl in H. }
+discriminate.
+Qed.
+
+Lemma N_div_0_r (n: N):
+  (n / 0 = 0)%N.
+Proof.
+now destruct n.
+Qed.
+
+Lemma Z_div_0_r (n: Z):
+  (n / 0 = 0)%Z.
+Proof.
+now destruct n.
+Qed.
+
+Lemma N_div_le (n: N) (d: N):
+  (n / d <= n)%N.
+Proof.
+assert (CN := N.eq_0_gt_0_cases n).
+assert (CD := N.eq_0_gt_0_cases d).
+case CN; intro. { subst. cbn. apply N.le_refl. }
+case CD; intro. { subst. rewrite N_div_0_r. now apply N.lt_le_incl. }
+assert (D: N.succ (N.pred d) = d).
+{ apply N.succ_pred_pos. assumption. }
+remember (N.pred d) as k. clear Heqk. subst.
+assert (CK := N.eq_0_gt_0_cases k).
+case CK; intro. { subst. cbn. now rewrite N.div_1_r. }
+apply N.lt_le_incl.
+apply N.div_lt. { assumption. }
+now apply N.lt_pred_lt_succ.
+Qed.
+
+Lemma Z_div_nonneg (a b: Z)
+                    (A: (0 <= a)%Z)
+                    (B: (0 <= b)%Z):
+  (0 <= a / b)%Z.
+Proof.
+destruct b. { rewrite Zdiv_0_r. apply Z.le_refl. }
+{ apply Z.div_pos; easy. }
+easy.
+Qed.
+
+Lemma Z_abs_div_le (a b: Z):
+  (Z.abs a / Z.abs b <= Z.abs a)%Z.
+Proof.
+assert(A := Z.abs_nonneg a).
+assert(B := Z.abs_nonneg b).
+apply Z2N.inj_le. { now apply Z_div_nonneg. }
+{ assumption. }
+rewrite Z2N.inj_div; try assumption.
+apply N_div_le.
+Qed.
+
+Lemma Z_abs_sgn (a b: Z):
+  Z.abs (Z.sgn a * b)%Z = match a with
+                          | 0%Z => 0%Z
+                          | _ => Z.abs b
+                          end.
+Proof.
+now destruct a, b.
+Qed.
+
+Lemma Z_sgn_abs (a: Z):
+  (Z.sgn a * Z.abs a)%Z = a.
+Proof.
+now destruct a.
+Qed.
+
+Lemma Z_add_nocarry_lor (a b: Z) (H: Z.land a b = 0%Z):
+  (a + b = Z.lor a b)%Z.
+Proof.
+rewrite Z.add_nocarry_lxor by assumption.
+apply Z.lxor_lor. assumption.
+Qed.
+
+Lemma Z_land_pow2_small (a b: Z) (A: (0 <= a < 2 ^ b)%Z) (B: (0 <= b)%Z):
+  Z.land a (2 ^ b) = 0%Z.
+Proof.
+rewrite Arith2.Z_land_pow2_shift by tauto.
+replace (Z.shiftr a b) with 0%Z. { cbn. apply Z.shiftl_0_l. }
+rewrite Z.shiftr_div_pow2 by tauto.
+symmetry. apply Z.div_small. exact A.
+Qed.
+
+Lemma Z_testbit_flag_mul_pow2 (f: bool) (k: Z) (K: (0 <= k)%Z):
+  Z.testbit ((if f then 1 else 0) * 2 ^ k) k = f.
+Proof.
+destruct f.
+{ rewrite Z.mul_1_l. apply Z.pow2_bits_true. assumption. }
+rewrite Z.mul_0_l. apply Z.bits_0.
+Qed.
+
+(* A version of Z.bits_above_log2 with a different bound. *)
+Lemma Z_testbit_small (a n: Z) (A: (0 <= a)%Z)
+                               (B: (a < 2 ^ n)%Z):
+  Z.testbit a n = false.
+Proof.
+destruct a. { apply Z.testbit_0_l. }
+{ apply Z.bits_above_log2. trivial. now apply Z.log2_lt_pow2. }
+exfalso. rewrite<- Z.leb_le in A. cbn in A. discriminate.
+Qed.
+
+(**************************************************************************)
+
+Lemma Z_pos_ne_0 (a: positive):
+  Z.pos a <> 0%Z.
+Proof.
+discriminate.
+Qed.
+
+Lemma Z_0_lt_pos (a: positive):
+  (0 < Z.pos a)%Z.
+Proof.
+rewrite<- Z.ltb_lt.
+trivial.
+Qed.
+
+Lemma Z_ceiling_via_floor (a b: Z) (B: (0 <= b)%Z):
+  (- ((- a) / b) = (a + b - 1) / b)%Z.
+Proof.
+destruct b as [|b|b]. { now repeat rewrite Z_div_0_r. }
+{
+  assert (D := Z.div_mod (-a) (Z.pos b) (Z_pos_ne_0 b)).
+  assert (E := Z.div_mod (a + Z.pos b - 1) (Z.pos b) (Z_pos_ne_0 b)).
+  assert (P := Z.mod_pos_bound (-a) (Z.pos b) (Z_0_lt_pos b)).
+  assert (Q := Z.mod_pos_bound (a + Z.pos b - 1) (Z.pos b) (Z_0_lt_pos b)).
+  nia.
+}
+rewrite<- Z.leb_le in B. discriminate.
+Qed.
+
+(**************************************************************************)
+
+Lemma Z_land_lxor_distr_l (a b c: Z):
+  Z.land (Z.lxor a b) c = Z.lxor (Z.land a c) (Z.land b c).
+Proof.
+apply Z.bits_inj. intro.
+repeat (rewrite Z.land_spec || rewrite Z.lxor_spec).
+destruct (Z.testbit a n); destruct (Z.testbit b n); destruct (Z.testbit c n); easy.
+Qed.
+
+Lemma Z_land_lxor_distr_r (a b c: Z):
+  Z.land a (Z.lxor b c) = Z.lxor (Z.land a b) (Z.land a c).
+Proof.
+apply Z.bits_inj. intro.
+repeat (rewrite Z.land_spec || rewrite Z.lxor_spec).
+destruct (Z.testbit a n); destruct (Z.testbit b n); destruct (Z.testbit c n); easy.
+Qed.
+
+(**************************************************************************)
+
+(* This is a version of Z.log2_lt_pow2 but a can be 0 and b cannot. *)
+Lemma Z_log2_lt_pow2 (a b: Z) (BA: (0 <= a)%Z) (BB: (0 < b)%Z):
+    (a < 2 ^ b <-> Z.log2 a < b)%Z.
+Proof.
+destruct a.
+{
+  cbn. assert (P: (0 < 2 ^ b)%Z). apply Z_0_lt_pow2. { apply Z.lt_le_incl. assumption. }
+  tauto.
+}
+{ apply Z.log2_lt_pow2. rewrite<- Z.ltb_lt. trivial. }
+rewrite<- Z.leb_le in BA. discriminate.
+Qed.
+
+(**************************************************************************)
+
+Lemma Z_mod_add_l (a b c m: Z)
+                  (H: (b mod m = c mod m)%Z):
+  ((a + b) mod m = (a + c) mod m)%Z.
+Proof.
+rewrite<- (Zplus_mod_idemp_r b a).
+rewrite<- (Zplus_mod_idemp_r c a).
+rewrite H.
+trivial.
+Qed.
+
+Lemma Z_mod_add_r (a b c m: Z)
+                  (H: (a mod m = b mod m)%Z):
+  ((a + c) mod m = (b + c) mod m)%Z.
+Proof.
+rewrite<- (Zplus_mod_idemp_l a c).
+rewrite<- (Zplus_mod_idemp_l b c).
+rewrite H.
+trivial.
+Qed.
+
+(**************************************************************************)
+
+Lemma Nat2N_inj_div (a b: nat):
+  N.of_nat (a / b) = (N.of_nat a / N.of_nat b)%N.
+Proof.
+destruct b. { cbn. now rewrite N_div_0_r. }
+assert (BNZ: S b <> 0) by discriminate.
+assert (D := Nat.div_mod a (S b) BNZ).
+remember (a / S b) as q.
+remember (a mod S b) as r.
+apply N.div_unique with (r := N.of_nat r).
+{
+  unfold N.lt.
+  rewrite<- Nat2N.inj_compare.
+  apply Nat.compare_lt_iff.
+  subst. apply (Nat.mod_upper_bound _ _ BNZ).
+}
+rewrite<- Nat2N.inj_mul.
+rewrite<- Nat2N.inj_add.
+now rewrite D.
+Qed.
+
+Lemma Nat2N_inj_mod (a b: nat) (ok: b <> 0):
+  N.of_nat (a mod b) = (N.of_nat a mod N.of_nat b)%N.
+Proof.
+destruct b. { contradiction. }
+rewrite Nat.mod_eq by discriminate.
+rewrite Nat2N.inj_sub.
+rewrite Nat2N.inj_mul.
+rewrite Nat2N_inj_div.
+symmetry. apply N.mod_eq.
+discriminate.
+Qed.
+
+(**************************************************************************)
+(** This is a strenghtening of Pos.size_nat_monotone from [p < q] to [p <= q]. *)
+Lemma Pos_size_nat_monotone (p q: positive) (LE: (p <= q)%positive):
+  (Pos.size_nat p <= Pos.size_nat q)%nat.
+Proof.
+remember (Pos.compare p q) as cmp. symmetry in Heqcmp. destruct cmp.
+{ apply Pos.compare_eq in Heqcmp. subst. apply Nat.le_refl. }
+{ apply Pos.size_nat_monotone. exact Heqcmp. }
+contradiction.
+Qed.
