Lib2/List2.v
@@ -1,0 +1,45 @@
+From Coq Require Import List Arith.
+
+Local Open Scope list_scope.
+
+Lemma skipn_skipn {A} (l: list A) (n m: nat):
+  skipn n (skipn m l) = skipn (n + m) l.
+Proof.
+revert n l.
+induction m, l; intros; try repeat rewrite skipn_nil; try easy.
+{ cbn. now rewrite Nat.add_0_r. }
+replace (n + S m) with (S (n + m)) by auto with arith.
+repeat rewrite skipn_cons.
+apply IHm.
+Qed.
+
+Lemma nth_hd_skipn {A} (l: list A) (n: nat):
+  nth_error l n = hd_error (skipn n l).
+Proof.
+revert l. induction n, l; try easy.
+cbn. apply IHn.
+Qed.
+
+Lemma nth_firstn {A} (l: list A) (d: A) (n k: nat) (L: k < n):
+  nth k (firstn n l) d = nth k l d.
+Proof.
+revert k n L. induction l; intros; cbn; destruct k, n; cbn; try easy.
+apply lt_S_n in L.
+apply (IHl _ _ L).
+Qed.
+
+Fixpoint list_eqb {A} (eqb: A -> A -> bool) (l l': list A)
+: bool
+:= match l with
+   | nil => match l' with
+            | nil => true
+            | _ => false
+            end
+   | h :: t => match l' with
+               | nil => false
+               | h' :: t' => if eqb h h'
+                               then list_eqb eqb t t'
+                               else false
+               end
+   end.
+
