Lib2/Logic2.v
@@ -1,0 +1,37 @@
+From Coq Require Setoid.
+
+Lemma b_false {b: bool} {P: Prop} (R: b = true <-> P):
+  b = false <-> ~P.
+Proof.
+split; intro H; destruct b; try intro T; try easy.
+{ apply R in T.  discriminate. }
+exfalso. apply H. apply R. trivial.
+Qed.
+
+Lemma relation_quad {TA TB TC TD: Type}
+                    {R1: TA -> TB -> Prop}
+                    {R2: TC -> TD -> Prop}
+                    {r1: TA -> TB -> bool}
+                    {r2: TC -> TD -> bool}
+                    (H1: forall x y, r1 x y = true <-> R1 x y)
+                    (H2: forall x y, r2 x y = true <-> R2 x y)
+                    (a: TA) (b: TB) (c: TC) (d: TD):
+  (r1 a b = r2 c d) <-> (R1 a b <-> R2 c d).
+Proof.
+split; intro K; repeat rewrite<- H;
+  remember (r1 a b) as rab; symmetry in Heqrab;
+  remember (r2 c d) as rcd; symmetry in Heqrcd;
+  destruct rab; destruct rcd;
+  try rewrite H1 in Heqrab; try rewrite H2 in Heqrcd; try easy.
+  {
+    split; intro Q.
+    { rewrite<- H1 in Q. rewrite Heqrab in Q. discriminate. }
+    { rewrite<- H2 in Q. rewrite Heqrcd in Q. discriminate. }
+  }
+  {
+    rewrite K in Heqrab. rewrite<- H2 in Heqrab.
+    rewrite<- Heqrab. rewrite<- Heqrcd. reflexivity.
+  }
+  rewrite<- K in Heqrcd. rewrite<- H1 in Heqrcd.
+  rewrite<- Heqrab. rewrite<- Heqrcd. reflexivity.
+Qed.
